sys-init/CreateObjects_SI.thy
@@ -14,49 +14,46 @@ imports
   Sep_Algebra.Sep_Util
   Sep_Algebra.Sep_Fold_Cancel
   Mapped_Separating_Conjunction
-  Lib.Guess_ExI
 begin
 
 lemma has_children_map_le:
   "\<lbrakk>cdl_cdt s \<subseteq>\<^sub>m cdl_cdt s'; has_children cap_ref s\<rbrakk>
   \<Longrightarrow> has_children cap_ref s'"
-  apply (clarsimp simp: has_children_def is_cdt_parent_def)
-  apply (rule_tac x=a in exI)
-  apply (rule_tac x=b in exI)
-  apply (clarsimp simp: map_le_def)
-  by (metis domIff option.distinct(1))
+  unfolding has_children_def is_cdt_parent_def
+  by (metis (no_types, opaque_lifting) domIff map_le_def not_None_eq)
 
 lemma retype_untyped_wp_no_children:
-  "\<lbrakk>default_object type sz minBound = Some new_object;
-    base_ptr \<in> all_available_ids;
-    free_cptr < 2 ^ si_cnode_size;
-    untyped_cptr < 2 ^ si_cnode_size;
-    sz < 2 ^ word_bits;
-    type \<noteq> UntypedType;
-    base_ptr = Min cover_ids\<rbrakk> \<Longrightarrow>
-    \<lbrace>\<lambda>s. \<guillemotleft>(si_cnode_id, unat untyped_cptr) \<mapsto>c UntypedCap dev cover_ids cover_ids \<and>*
-      (\<And>* obj_id \<in> all_available_ids. (obj_id \<mapsto>o Untyped)) \<and>*
-      (si_cnode_id, unat free_cptr) \<mapsto>c NullCap \<and>*
-      si_tcb_id \<mapsto>f root_tcb \<and>*
-      (si_tcb_id, tcb_pending_op_slot) \<mapsto>c RunningCap \<and>*
-      (si_tcb_id, tcb_cspace_slot) \<mapsto>c si_cspace_cap \<and>*
-      si_cnode_id \<mapsto>f CNode (empty_cnode si_cnode_size) \<and>*
-      (si_cnode_id, unat seL4_CapInitThreadCNode) \<mapsto>c si_cnode_cap \<and>* R\<guillemotright> s \<and>
-      \<not>has_children (si_cnode_id,unat untyped_cptr) (kernel_state s)\<rbrace>
-
+  "\<lbrakk> default_object type sz minBound = Some new_object;
+     base_ptr \<in> all_available_ids;
+     free_cptr < 2 ^ si_cnode_size;
+     untyped_cptr < 2 ^ si_cnode_size;
+     sz < 2 ^ word_bits;
+     type \<noteq> UntypedType;
+     base_ptr = Min cover_ids \<rbrakk> \<Longrightarrow>
+    \<lbrace>\<lambda>s. \<guillemotleft> (si_cnode_id, unat untyped_cptr) \<mapsto>c UntypedCap dev cover_ids cover_ids \<and>*
+           (\<And>* obj_id \<in> all_available_ids. (obj_id \<mapsto>o Untyped)) \<and>*
+           (si_cnode_id, unat free_cptr) \<mapsto>c NullCap \<and>*
+           si_tcb_id \<mapsto>f root_tcb \<and>*
+           (si_tcb_id, tcb_pending_op_slot) \<mapsto>c RunningCap \<and>*
+           (si_tcb_id, tcb_cspace_slot) \<mapsto>c si_cspace_cap \<and>*
+           si_cnode_id \<mapsto>f CNode (empty_cnode si_cnode_size) \<and>*
+           (si_cnode_id, unat seL4_CapInitThreadCNode) \<mapsto>c si_cnode_cap \<and>* R\<guillemotright> s \<and>
+         \<not>has_children (si_cnode_id,unat untyped_cptr) (kernel_state s)\<rbrace>
     retype_untyped free_cptr untyped_cptr type sz
-
-   \<lbrace>\<lambda>rv s.
-    \<guillemotleft>(si_cnode_id, unat untyped_cptr) \<mapsto>c UntypedCap dev cover_ids (update_range cover_ids (base_ptr) (unat (base_ptr + 2 ^ obj_bits_cdl type sz - base_ptr))) \<and>*
-    (\<And>* obj_id \<in> all_available_ids - {base_ptr}. (obj_id \<mapsto>o Untyped)) \<and>*
-     base_ptr \<mapsto>o new_object \<and>*
-    (si_cnode_id, unat free_cptr) \<mapsto>c default_cap type {base_ptr} sz dev \<and>*
-     si_tcb_id \<mapsto>f root_tcb \<and>*
-    (si_tcb_id, tcb_pending_op_slot) \<mapsto>c RunningCap \<and>*
-    (si_tcb_id, tcb_cspace_slot) \<mapsto>c si_cspace_cap \<and>*
-     si_cnode_id \<mapsto>f CNode (empty_cnode si_cnode_size) \<and>*
-    (si_cnode_id, unat seL4_CapInitThreadCNode) \<mapsto>c si_cnode_cap \<and>* R \<guillemotright> s \<and>
-    has_children (si_cnode_id,unat untyped_cptr) (kernel_state s)\<rbrace>"
+    \<lbrace>\<lambda>_ s.
+       \<guillemotleft> (si_cnode_id, unat untyped_cptr) \<mapsto>c
+            UntypedCap dev cover_ids
+                       (update_range cover_ids (base_ptr)
+                         (unat (base_ptr + 2 ^ obj_bits_cdl type sz - base_ptr))) \<and>*
+         (\<And>* obj_id \<in> all_available_ids - {base_ptr}. (obj_id \<mapsto>o Untyped)) \<and>*
+         base_ptr \<mapsto>o new_object \<and>*
+         (si_cnode_id, unat free_cptr) \<mapsto>c default_cap type {base_ptr} sz dev \<and>*
+          si_tcb_id \<mapsto>f root_tcb \<and>*
+         (si_tcb_id, tcb_pending_op_slot) \<mapsto>c RunningCap \<and>*
+         (si_tcb_id, tcb_cspace_slot) \<mapsto>c si_cspace_cap \<and>*
+         si_cnode_id \<mapsto>f CNode (empty_cnode si_cnode_size) \<and>*
+         (si_cnode_id, unat seL4_CapInitThreadCNode) \<mapsto>c si_cnode_cap \<and>* R \<guillemotright> s \<and>
+       has_children (si_cnode_id,unat untyped_cptr) (kernel_state s)\<rbrace>"
   apply (rule hoare_name_pre_state)
   apply (subgoal_tac "si_cspace_cap=si_cnode_cap", simp)
    apply (unfold retype_untyped_def)
@@ -70,13 +67,15 @@ lemma retype_untyped_wp_no_children:
                                                obj_range=cover_ids and
                                                tcb="obj_tcb root_tcb"]])
                apply (fastforce)+
-         apply (assumption | simp add: unat_of_nat32 | rule offset_slot' [symmetric] guard_equal_si_cnode_cap)+
+         apply (assumption
+                | simp add: unat_of_nat32
+                | rule offset_slot' [symmetric] guard_equal_si_cnode_cap)+
     apply (clarsimp)
     apply (clarsimp simp: offset_slot')
     apply (sep_erule_concl refl_imp)+
     apply sep_solve
    apply (clarsimp simp: unat_of_nat32 offset_slot')
-   apply (sep_solve)
+   apply sep_solve
   apply (clarsimp simp: si_cspace_cap_def si_cnode_cap_def)
   done
 
@@ -99,44 +98,47 @@ lemma retype_untyped_wp_has_children:
       si_cnode_id \<mapsto>f CNode (empty_cnode si_cnode_size) \<and>*
       (si_cnode_id, unat seL4_CapInitThreadCNode) \<mapsto>c si_cnode_cap \<and>* R\<guillemotright> s \<and>
       has_children (si_cnode_id,unat untyped_cptr) (kernel_state s)\<rbrace>
-
-     retype_untyped free_cptr untyped_cptr type sz
-
-   \<lbrace>\<lambda>rv s.
-    \<guillemotleft>(si_cnode_id, unat untyped_cptr) \<mapsto>c UntypedCap dev cover_ids (update_range cover_ids (base_ptr) (unat (alignUp next_ptr (obj_bits_cdl type sz) + 2 ^ obj_bits_cdl type sz - base_ptr))) \<and>*
-    (\<And>* obj_id \<in> all_available_ids - {alignUp next_ptr (obj_bits_cdl type sz)}. (obj_id \<mapsto>o Untyped)) \<and>*
-     alignUp next_ptr (obj_bits_cdl type sz) \<mapsto>o new_object \<and>*
-    (si_cnode_id, unat free_cptr) \<mapsto>c default_cap type {alignUp next_ptr (obj_bits_cdl type sz)} sz dev \<and>*
-     si_tcb_id \<mapsto>f root_tcb \<and>*
-    (si_tcb_id, tcb_pending_op_slot) \<mapsto>c RunningCap \<and>*
-    (si_tcb_id, tcb_cspace_slot) \<mapsto>c si_cspace_cap \<and>*
-     si_cnode_id \<mapsto>f CNode (empty_cnode si_cnode_size) \<and>*
-    (si_cnode_id, unat seL4_CapInitThreadCNode) \<mapsto>c si_cnode_cap \<and>* R \<guillemotright> s \<and>
-    has_children (si_cnode_id,unat untyped_cptr) (kernel_state s)\<rbrace>"
+    retype_untyped free_cptr untyped_cptr type sz
+    \<lbrace>\<lambda>rv s.
+     \<guillemotleft>(si_cnode_id, unat untyped_cptr) \<mapsto>c
+        UntypedCap dev cover_ids
+                   (update_range cover_ids (base_ptr)
+                      (unat (alignUp next_ptr (obj_bits_cdl type sz) +
+                             2 ^ obj_bits_cdl type sz - base_ptr))) \<and>*
+      (\<And>* obj_id \<in> all_available_ids - {alignUp next_ptr (obj_bits_cdl type sz)}.
+         (obj_id \<mapsto>o Untyped)) \<and>*
+      alignUp next_ptr (obj_bits_cdl type sz) \<mapsto>o new_object \<and>*
+      (si_cnode_id, unat free_cptr) \<mapsto>c
+        default_cap type {alignUp next_ptr (obj_bits_cdl type sz)} sz dev \<and>*
+      si_tcb_id \<mapsto>f root_tcb \<and>*
+      (si_tcb_id, tcb_pending_op_slot) \<mapsto>c RunningCap \<and>*
+      (si_tcb_id, tcb_cspace_slot) \<mapsto>c si_cspace_cap \<and>*
+      si_cnode_id \<mapsto>f CNode (empty_cnode si_cnode_size) \<and>*
+      (si_cnode_id, unat seL4_CapInitThreadCNode) \<mapsto>c si_cnode_cap \<and>* R \<guillemotright> s \<and>
+      has_children (si_cnode_id,unat untyped_cptr) (kernel_state s)\<rbrace>"
   apply (subgoal_tac "si_cspace_cap=si_cnode_cap", simp)
    apply (unfold retype_untyped_def)
    apply (wp)
      apply (clarsimp simp: comp_def, wp)
     apply (rule hoare_chain[OF seL4_Untyped_Retype_sep[where free_range = available_ids and
                                                tot_free_range = all_available_ids and
-                                               root_cnode_cap= si_cnode_cap and
-                                               root_size=si_cnode_size and
-                                               dev=dev and
+                                               root_cnode_cap = si_cnode_cap and
+                                               root_size = si_cnode_size and
+                                               dev = dev and
                                                obj = new_object and
-                                               obj_range=cover_ids and
-                                               tcb="obj_tcb root_tcb"]])
+                                               obj_range = cover_ids and
+                                               tcb = "obj_tcb root_tcb"]])
              apply (fastforce)+
-         apply (assumption | simp add: unat_of_nat32 | rule offset_slot' [symmetric] guard_equal_si_cnode_cap)+
+         apply (simp add: unat_of_nat32 | rule offset_slot'[symmetric] guard_equal_si_cnode_cap)+
     apply (clarsimp)
     apply (clarsimp simp: offset_slot')
     apply (sep_erule_concl refl_imp)+
     apply (clarsimp)
     apply (assumption)
-   apply (assumption | simp add: unat_of_nat32 | rule offset_slot' [symmetric] guard_equal_si_cnode_cap)+
-   apply (clarsimp, intro conjI impI)
-    apply (clarsimp simp: offset_slot')+
-    apply (sep_solve)
-   apply (clarsimp simp: offset_slot' si_cspace_cap_def si_cnode_cap_def)+
+   apply (simp add: unat_of_nat32 | rule offset_slot'[symmetric] guard_equal_si_cnode_cap)+
+   apply (clarsimp simp: keep_if_cond offset_slot')
+   apply sep_solve
+  apply (clarsimp simp: si_cspace_cap_def si_cnode_cap_def)
   done
 
 lemma untyped_cap_eq:
@@ -144,31 +146,31 @@ lemma untyped_cap_eq:
   by (clarsimp simp: cap_type_def cap_free_ids_def split: cdl_cap.splits)
 
 lemma create_object_first:
-  "cdl_objects spec child = Some child_obj \<Longrightarrow>
-   default_object (object_type child_obj) (object_size_bits child_obj) minBound = Some default_child \<Longrightarrow>
-   si_caps child = Some free_cptr \<Longrightarrow>
-   the (si_caps child) < 2 ^ si_cnode_size \<Longrightarrow>
-   parent < 2 ^ si_cnode_size \<Longrightarrow>
-   object_type child_obj \<noteq> UntypedType \<Longrightarrow>
-   object_size_bits child_obj < 2 ^ word_bits \<Longrightarrow>
-   obj_size = (obj_bits_cdl (object_type child_obj) (object_size_bits child_obj)) \<Longrightarrow>
-   obj_size < word_size \<Longrightarrow>
-   t child = Some (alignUp base_ptr obj_size) \<Longrightarrow>
-   cover_ids \<noteq> {} \<Longrightarrow>
-   base_ptr = Min cover_ids \<Longrightarrow>
-   base_ptr \<le> base_ptr + 2 ^ obj_size \<Longrightarrow>
-   is_aligned base_ptr obj_size \<Longrightarrow>
+  "\<lbrakk> cdl_objects spec child = Some child_obj;
+     default_object (object_type child_obj) (object_size_bits child_obj) minBound =
+       Some default_child;
+     si_caps child = Some free_cptr;
+     the (si_caps child) < 2 ^ si_cnode_size;
+     parent < 2 ^ si_cnode_size;
+     object_type child_obj \<noteq> UntypedType;
+     object_size_bits child_obj < 2 ^ word_bits;
+     obj_size = (obj_bits_cdl (object_type child_obj) (object_size_bits child_obj));
+     obj_size < word_size;
+     t child = Some (alignUp base_ptr obj_size);
+     cover_ids \<noteq> {};
+     base_ptr = Min cover_ids;
+     base_ptr \<le> base_ptr + 2 ^ obj_size;
+     is_aligned base_ptr obj_size \<rbrakk> \<Longrightarrow>
    \<lbrace> \<guillemotleft>si_objects \<and>*
       si_null_cap_at t si_caps spec child \<and>*
       (the (t child)) \<mapsto>o Untyped \<and>*
       (si_cnode_id, unat parent) \<mapsto>c UntypedCap dev cover_ids cover_ids \<and>* R\<guillemotright> \<rbrace>
-
-     create_object spec si_caps parent child
-
+   create_object spec si_caps parent child
    \<lbrace>\<lambda>_. \<guillemotleft>si_cap_at t si_caps spec dev child \<and>*
-          si_objects \<and>* (the (t child)) \<mapsto>o default_child \<and>*
-          (si_cnode_id, unat parent) \<mapsto>c UntypedCap dev cover_ids (cover_ids - {..<base_ptr + 2 ^ obj_size}) \<and>* R\<guillemotright> \<rbrace>"
-  apply (rule hoare_name_pre_state)
+         si_objects \<and>* (the (t child)) \<mapsto>o default_child \<and>*
+         (si_cnode_id, unat parent) \<mapsto>c
+           UntypedCap dev cover_ids (cover_ids - {..<base_ptr + 2 ^ obj_size}) \<and>* R\<guillemotright> \<rbrace>"
+  apply (rule hoare_name_pre_state, rename_tac s)
   apply (case_tac "has_children (si_cnode_id, unat parent) (kernel_state s)")
    apply (clarsimp simp: create_object_def assert_opt_def, wp)
     apply (rule hoare_strengthen_post[OF retype_untyped_wp_has_children[where dev=dev and
@@ -202,30 +204,29 @@ lemma create_object_first:
   done
 
 lemma create_object_has_children:
-  "cdl_objects spec child = Some child_obj \<Longrightarrow>
-   default_object (object_type child_obj) (object_size_bits child_obj) minBound = Some default_child \<Longrightarrow>
-   si_caps child = Some free_cptr \<Longrightarrow>
-   the (si_caps child) < 2 ^ si_cnode_size \<Longrightarrow>
-   parent < 2 ^ si_cnode_size \<Longrightarrow>
-   object_type child_obj \<noteq> UntypedType \<Longrightarrow>
-   object_size_bits child_obj < 2 ^ word_bits \<Longrightarrow>
-   obj_size = (obj_bits_cdl (object_type child_obj) (object_size_bits child_obj)) \<Longrightarrow>
-   obj_size < word_size \<Longrightarrow>
-   t child = Some (alignUp base_ptr obj_size) \<Longrightarrow>
-   cover_ids \<noteq> {} \<Longrightarrow>
-   available_ids \<noteq> {} \<Longrightarrow>
-   base_ptr = Min cover_ids \<Longrightarrow>
-   base_ptr \<le> base_ptr + 2 ^ obj_size \<Longrightarrow>
-   is_aligned base_ptr obj_size \<Longrightarrow>
+  "\<lbrakk> cdl_objects spec child = Some child_obj;
+     default_object (object_type child_obj) (object_size_bits child_obj) minBound =
+       Some default_child;
+     si_caps child = Some free_cptr;
+     the (si_caps child) < 2 ^ si_cnode_size;
+     parent < 2 ^ si_cnode_size;
+     object_type child_obj \<noteq> UntypedType;
+     object_size_bits child_obj < 2 ^ word_bits;
+     obj_size = (obj_bits_cdl (object_type child_obj) (object_size_bits child_obj));
+     obj_size < word_size;
+     t child = Some (alignUp base_ptr obj_size);
+     cover_ids \<noteq> {};
+     available_ids \<noteq> {};
+     base_ptr = Min cover_ids;
+     base_ptr \<le> base_ptr + 2 ^ obj_size;
+     is_aligned base_ptr obj_size \<rbrakk> \<Longrightarrow>
    \<lbrace> \<guillemotleft>si_objects \<and>*
       si_null_cap_at t si_caps spec child \<and>*
       (the (t child)) \<mapsto>o Untyped \<and>*
       (si_cnode_id, unat parent) \<mapsto>c UntypedCap dev cover_ids cover_ids \<and>* R\<guillemotright> \<rbrace>
-
-     create_object spec si_caps parent child
-
+   create_object spec si_caps parent child
    \<lbrace>\<lambda>_ s. has_children (si_cnode_id, unat parent) (kernel_state s) \<rbrace>"
-  apply (rule hoare_name_pre_state)
+  apply (rule hoare_name_pre_state, rename_tac s)
   apply (case_tac "has_children (si_cnode_id, unat parent) (kernel_state s)")
    apply (clarsimp simp: create_object_def assert_opt_def, wp)
     apply (rule hoare_strengthen_post[OF retype_untyped_wp_has_children[where dev=dev and
@@ -254,32 +255,34 @@ lemma create_object_has_children:
   done
 
 lemma create_object_rest:
-  "cdl_objects spec child = Some child_obj \<Longrightarrow>
-   default_object (object_type child_obj) (object_size_bits child_obj) minBound = Some default_child \<Longrightarrow>
-   si_caps child = Some free_cptr \<Longrightarrow>
-   the (si_caps child) < 2 ^ si_cnode_size \<Longrightarrow>
-   parent < 2 ^ si_cnode_size \<Longrightarrow>
-   object_type child_obj \<noteq> UntypedType \<Longrightarrow>
-   object_size_bits child_obj < 2 ^ word_bits \<Longrightarrow>
-   obj_size = (obj_bits_cdl (object_type child_obj) (object_size_bits child_obj)) \<Longrightarrow>
-   obj_size < word_size \<Longrightarrow>
-   t child = Some (alignUp next_ptr obj_size) \<Longrightarrow>
-   cover_ids \<noteq> {} \<Longrightarrow>
-   available_ids \<noteq> {} \<Longrightarrow>
-   next_ptr = Min available_ids \<Longrightarrow>
-   base_ptr = Min cover_ids \<Longrightarrow>
+  "\<lbrakk> cdl_objects spec child = Some child_obj;
+     default_object (object_type child_obj) (object_size_bits child_obj) minBound =
+       Some default_child;
+     si_caps child = Some free_cptr;
+     the (si_caps child) < 2 ^ si_cnode_size;
+     parent < 2 ^ si_cnode_size;
+     object_type child_obj \<noteq> UntypedType;
+     object_size_bits child_obj < 2 ^ word_bits;
+     obj_size = (obj_bits_cdl (object_type child_obj) (object_size_bits child_obj));
+     obj_size < word_size;
+     t child = Some (alignUp next_ptr obj_size);
+     cover_ids \<noteq> {};
+     available_ids \<noteq> {};
+     next_ptr = Min available_ids;
+     base_ptr = Min cover_ids \<rbrakk> \<Longrightarrow>
    \<lbrace> \<guillemotleft>si_objects \<and>*
       si_null_cap_at t si_caps spec child \<and>*
       (the (t child)) \<mapsto>o Untyped \<and>*
       (si_cnode_id, unat parent) \<mapsto>c UntypedCap dev cover_ids available_ids \<and>* R\<guillemotright> and
       (\<lambda>s. has_children (si_cnode_id, unat parent) (kernel_state s)) \<rbrace>
-
-     create_object spec si_caps parent child
-
+   create_object spec si_caps parent child
    \<lbrace>\<lambda>_. \<guillemotleft>si_cap_at t si_caps spec dev child \<and>*
-          si_objects \<and>* (the (t child)) \<mapsto>o default_child \<and>*
-          (si_cnode_id, unat parent) \<mapsto>c UntypedCap dev cover_ids (update_range cover_ids base_ptr (unat (the (t child) + 2 ^ obj_size - base_ptr))) \<and>* R\<guillemotright> and
-          (\<lambda>s. has_children (si_cnode_id, unat parent) (kernel_state s)) \<rbrace>"
+         si_objects \<and>* (the (t child)) \<mapsto>o default_child \<and>*
+         (si_cnode_id, unat parent) \<mapsto>c
+           UntypedCap dev cover_ids
+                      (update_range cover_ids base_ptr
+                                    (unat (the (t child) + 2 ^ obj_size - base_ptr))) \<and>* R\<guillemotright> and
+         (\<lambda>s. has_children (si_cnode_id, unat parent) (kernel_state s)) \<rbrace>"
   apply (rule hoare_name_pre_state)
   apply (clarsimp simp: create_object_def assert_opt_def, wp)
    apply (rule hoare_strengthen_post[OF retype_untyped_wp_has_children[where dev=dev and
@@ -300,19 +303,21 @@ lemma create_object_rest:
   done
 
 lemma sep_hoare_fold_mapM_x_inv:
-  "(\<And>R x. x \<in> set xs \<Longrightarrow> \<lbrace>\<lambda>s. (P x \<and>* R) (sep_lift s) \<and> P' s\<rbrace> f x \<lbrace>\<lambda>_ s. (Q x \<and>* R) (sep_lift s) \<and> P' s\<rbrace>)
-    \<Longrightarrow> \<lbrace>\<lambda>s. (sep_fold P Q R xs) (sep_lift s) \<and> P' s \<rbrace> mapM_x f xs \<lbrace>\<lambda>_ s. R (sep_lift s)\<rbrace>"
+  "(\<And>R x. x \<in> set xs \<Longrightarrow>
+          \<lbrace>\<lambda>s. (P x \<and>* R) (sep_lift s) \<and> P' s\<rbrace> f x \<lbrace>\<lambda>_ s. (Q x \<and>* R) (sep_lift s) \<and> P' s\<rbrace>)
+   \<Longrightarrow> \<lbrace>\<lambda>s. (sep_fold P Q R xs) (sep_lift s) \<and> P' s \<rbrace> mapM_x f xs \<lbrace>\<lambda>_ s. R (sep_lift s)\<rbrace>"
   apply (clarsimp simp: sep_fold_def)
   apply (induct xs arbitrary: R)
-   apply (clarsimp simp: mapM_x_def sequence_x_def)+
+   apply (clarsimp simp: mapM_x_def sequence_x_def)
    apply wp
-   apply (clarsimp)
+   apply clarsimp
+  apply (rename_tac x xs R)
   apply (simp add: mapM_x_Cons, wp)
     apply assumption+
    apply atomize
    apply (erule allE)
    apply (erule allE)
-   apply (erule_tac x=a in allE)
+   apply (erule_tac x=x in allE)
    apply (drule mp)
     apply (clarsimp)
    apply (rule hoare_chain)
@@ -322,132 +327,146 @@ lemma sep_hoare_fold_mapM_x_inv:
   apply clarsimp
   done
 
-lemma si_null_cap_at_cong: "t a = v a \<Longrightarrow> si_null_cap_at t si_caps spec a = si_null_cap_at (\<lambda>x. v x) si_caps spec a"
-  apply (clarsimp simp: si_null_cap_at_def)
-  done
+lemma si_null_cap_at_cong:
+  "t a = v a \<Longrightarrow> si_null_cap_at t si_caps spec a = si_null_cap_at (\<lambda>x. v x) si_caps spec a"
+  by (clarsimp simp: si_null_cap_at_def)
 
-lemma si_cap_at_cong: "t a = v a \<Longrightarrow> si_cap_at t si_caps spec dev a = si_cap_at (\<lambda>x. v x) si_caps spec dev a"
-  apply (clarsimp simp: si_cap_at_def)
-  done
+lemma si_cap_at_cong:
+  "t a = v a \<Longrightarrow> si_cap_at t si_caps spec dev a = si_cap_at (\<lambda>x. v x) si_caps spec dev a"
+  by (clarsimp simp: si_cap_at_def)
 
-lemma [simp]: "x + Map.empty = x" by (rule ext, clarsimp simp: plus_fun_def plus_option_def split: option.splits)
+lemma plus_empty_map[simp]: (* FIXME: move to Lib *)
+  "x + Map.empty = x"
+  "Map.empty + x = x"
+  by (rule ext, clarsimp simp: plus_fun_def plus_option_def split: option.splits)+
 
-lemma sub_neq_zero_le: "y < (x :: machine_word) \<Longrightarrow> x - y \<noteq> 0"
- by (clarsimp)
+lemma word_sub_neq_zero_le: (* FIXME: move to WordLib *)
+  "y < x \<Longrightarrow> x - y \<noteq> 0" for x :: "'a::len word"
+  by simp
 
-lemma Some_the: "x = Some y \<Longrightarrow> the x = y"
- by (clarsimp)
+lemma Some_the:
+  "x = Some y \<Longrightarrow> the x = y"
+  by simp
 
-definition "partial (f) (x :: 'a :: zero) = (if x = 0 then \<box> else f x)"
+(* FIXME: delete all this and prove sep_fold_simplify_loop more directly. *)
+(* f is a function from a type with 0 to separation logic predicates.
+   "partial f" always returns the empty heap for 0. *)
+definition partial :: "('a::zero \<Rightarrow> 'b::sep_algebra \<Rightarrow> bool) \<Rightarrow> 'a \<Rightarrow> 'b \<Rightarrow> bool" where
+  "partial f x = (if x = 0 then \<box> else f x)"
 
+(* To use lists with the partial function above, instantiate the list type as an additive monoid,
+   i.e. define + and 0 and observe associativity and 0 as the neutral element, where + is append
+   and 0 is the empty list. Now that lists have 0, "partial f" applies to lists and will return
+   the empty heap predicate for the empty list. All this setup gives us a default case for empty
+   lists in the rule sep_fold_simplify_loop below where "hd" can now be used as if it was a
+   partial function. *)
 instantiation list :: (type) monoid_add
 begin
-  definition "zero_list = []"
-  definition "plus_list (x :: 'a list) y = x @ y"
+
+definition "zero_list = []"
+definition "plus_list (x :: 'a list) y = x @ y"
+
 instance
- apply (intro_classes;clarsimp simp: zero_list_def plus_list_def)
-done
+  by (intro_classes;clarsimp simp: zero_list_def plus_list_def)
+
 end
 
-lemma [simp]: "partial (P \<circ> f) (x # xs) = (P o f) (x # xs)"
- apply (clarsimp simp: partial_def zero_list_def)
-done
+lemma partial_Cons[simp]:
+  "partial (P \<circ> f) (x # xs) = (P o f) (x # xs)"
+  by (clarsimp simp: partial_def zero_list_def)
 
-lemma [simp]: "partial (P \<circ> f) [] = \<box>"
- apply (clarsimp simp: partial_def zero_list_def)
-done
+lemma partial_Nil[simp]:
+  "partial (P \<circ> f) [] = \<box>"
+  by (clarsimp simp: partial_def zero_list_def)
 
-
-
-
-
-
-
-lemma induct_list: "\<lbrakk>P []; \<And>x. P [x];  \<And>x y xs. P (y#xs) \<Longrightarrow> P ([x,y] @ xs)\<rbrakk> \<Longrightarrow> P xs"
- apply (induct xs; clarsimp)
- apply (case_tac xs; clarsimp)
-done
-
-
-lemma sep_fold_simplify_loop: "distinct xs  \<Longrightarrow> (\<And>x y s. y \<in>set xs \<Longrightarrow> previous y xs = Some x \<Longrightarrow> Q x s \<Longrightarrow> P y s) \<Longrightarrow>
-       (partial (P o hd) xs \<and>* (sep_fold P' Q' ((partial (Q o last) xs) \<longrightarrow>* R) xs)) s \<Longrightarrow>
-       (sep_fold (\<lambda>x. P x \<and>* P' x) (\<lambda>x. Q x \<and>* Q' x) R xs) s "
- apply (induct xs  arbitrary: s R rule: induct_list ; clarsimp simp: sep_fold_def)
- apply (sep_solve)
- apply (sep_cancel)+
- apply (sep_solve)
- apply (sep_cancel)+
- apply (drule_tac x=sc in meta_spec)
- apply (drule_tac x=R in meta_spec)
- apply (atomize)
- apply (erule impE)
- apply (clarsimp)
- apply (intro impI conjI; clarsimp? )
- apply (erule_tac x=xa in allE)
- apply (erule_tac x=y in allE)
- apply (erule_tac x=s in allE)
- apply (clarsimp)
-  using not_in_previous' apply fastforce
- apply (erule_tac x=xa in allE)
- apply (erule_tac x=ya in allE)
- apply (erule_tac x=s in allE)
- apply (clarsimp)
-  apply presburger
-  apply (erule mp)
- apply (sep_mp)
- apply (sep_cancel)+
- apply (clarsimp)
-done
-
-definition "default_object_in spec ptr =
-  (let obj = (the (cdl_objects spec ptr)) in the (default_object (object_type obj) (object_size_bits obj) minBound))"
-
-lemma default_object_some_default: "cdl_objects spec ptr = Some obj \<Longrightarrow>
-       default_object (object_type obj) (object_size_bits obj) minBound = Some (default_object_in spec ptr)"
-  apply (clarsimp simp: default_object_in_def)
-  by (cases obj; clarsimp simp: default_object_def object_type_def)
-
-
-
-lemma the_some_cdl_objects[elim]: "cdl_objects spec ptr = Some obj \<Longrightarrow>  P (the (cdl_objects spec ptr))  = P obj"
-  by (clarsimp)
-
-lemma default_object_is_object_empty: "(ptr \<mapsto>o default_object_in spec a) s \<Longrightarrow> cdl_objects spec a = Some obj \<Longrightarrow>
-       object_domain obj = minBound \<Longrightarrow> t a = Some ptr \<Longrightarrow>
-       (object_empty spec t a) s"
- by (clarsimp simp: object_empty_def object_initialised_general_def object_default_state_def default_object_in_def)
-
-lemma extD1: "P = Q \<Longrightarrow> P x \<Longrightarrow> Q x"
- by (erule subst)
-
-
-
-
-
-
-lemma Min_diff_upt: "finite S \<Longrightarrow> v \<in> S \<Longrightarrow> Min (S - {..<v}) =  v"
-  apply (rule Min_eqI; clarsimp)
-  apply simp
+lemma two_induct_list:
+  "\<lbrakk>P []; \<And>x. P [x];  \<And>x y xs. P (y#xs) \<Longrightarrow> P ([x,y] @ xs)\<rbrakk> \<Longrightarrow> P xs"
+  apply (induct xs; clarsimp)
+  apply (case_tac xs; clarsimp)
   done
 
+lemma sep_fold_simplify_loop:
+  "\<lbrakk> distinct xs; \<And>x y s. y \<in>set xs \<Longrightarrow> previous y xs = Some x \<Longrightarrow> Q x s \<Longrightarrow> P y s;
+     (partial (P o hd) xs \<and>* (sep_fold P' Q' ((partial (Q o last) xs) \<longrightarrow>* R) xs)) s \<rbrakk> \<Longrightarrow>
+   (sep_fold (\<lambda>x. P x \<and>* P' x) (\<lambda>x. Q x \<and>* Q' x) R xs) s"
+  apply (induct xs  arbitrary: s R rule: two_induct_list; clarsimp simp: sep_fold_def)
+    apply (sep_solve)
+   apply (sep_cancel)+
+   apply (sep_solve)
+  apply (rename_tac R)
+  apply (sep_cancel)+
+  apply (rename_tac sc)
+  apply (drule_tac x=sc in meta_spec)
+  apply (drule_tac x=R in meta_spec)
+  apply (atomize)
+  apply (erule impE)
+   apply (clarsimp)
+   apply (intro impI conjI, clarsimp)
+    apply (fastforce dest!: not_in_previous')
+   apply metis
+  apply (erule mp)
+  apply (sep_mp)
+  apply (sep_cancel)+
+  apply (clarsimp)
+  done
+
+definition
+  "default_object_in spec ptr \<equiv>
+     let obj = the (cdl_objects spec ptr)
+     in the (default_object (object_type obj) (object_size_bits obj) minBound)"
+
+lemma default_object_some_default:
+  "cdl_objects spec ptr = Some obj \<Longrightarrow>
+   default_object (object_type obj) (object_size_bits obj) minBound =
+     Some (default_object_in spec ptr)"
+  unfolding default_object_in_def
+  by (cases obj; clarsimp simp: default_object_def object_type_def)
+
+lemma the_some_cdl_objects[elim]:
+  "cdl_objects spec ptr = Some obj \<Longrightarrow> P (the (cdl_objects spec ptr)) = P obj"
+  by clarsimp
+
+lemma default_object_is_object_empty:
+  "\<lbrakk> (ptr \<mapsto>o default_object_in spec a) s; cdl_objects spec a = Some obj;
+     object_domain obj = minBound; t a = Some ptr \<rbrakk>\<Longrightarrow>
+   object_empty spec t a s"
+  by (clarsimp simp: object_empty_def object_initialised_general_def object_default_state_def
+                     default_object_in_def)
+
+lemmas fun_congD1 = fun_cong[THEN iffD1]
+
+lemma Min_diff_upt:
+  "\<lbrakk> finite S; v \<in> S \<rbrakk> \<Longrightarrow> Min (S - {..<v}) =  v"
+  by (auto intro: Min_eqI)
+
 lemma create_children_wp:
-  assumes
-    increasing_allocations:"list_all (\<lambda>child. previous child children \<noteq> None \<longrightarrow> Min cover_ids < the (allocate (Min cover_ids) spec children child)) children" and
-    aligned_no_wrap:"list_all (\<lambda>child.  Min cover_ids \<le> the (aligned_allocations spec (Min cover_ids) children child) + 2 ^ (spec_object_size spec child )) children"
+  assumes increasing_allocations:
+    "list_all (\<lambda>child. previous child children \<noteq> None \<longrightarrow>
+     Min cover_ids < the (allocate (Min cover_ids) spec children child)) children"
+  assumes aligned_no_wrap:
+    "list_all (\<lambda>child. Min cover_ids \<le> the (aligned_allocations spec (Min cover_ids) children child)
+                                       + 2 ^ (spec_object_size spec child ))
+              children"
+  defines the_obj_def[simp]:
+    "the_obj \<equiv> \<lambda>p. the (cdl_objects spec p)"
+  defines the_obits_def[simp]:
+    "the_obits \<equiv> \<lambda>p. object_size_bits (the_obj p)"
+  defines the_tbits_def[simp]:
+    "the_tbits \<equiv> \<lambda>p. obj_bits_cdl (object_type (the_obj p)) (the_obits p)"
   shows
-    "\<forall>x \<in> set children. t x = (aligned_allocations spec (Min cover_ids) children) x \<Longrightarrow>
-     cover_ids \<noteq> {} \<Longrightarrow>
-     finite cover_ids \<Longrightarrow>
-     distinct children \<Longrightarrow>
-     \<forall>obj\<in>ran (cdl_objects spec). object_domain obj = minBound \<Longrightarrow>
-     list_all (\<lambda>child. the (allocate (Min cover_ids) spec children child) \<in> cover_ids ) children \<Longrightarrow>
-     list_all (\<lambda>child. si_caps child \<noteq> None \<and> the (si_caps child) < 2 ^ si_cnode_size) children \<Longrightarrow>
-     list_all (\<lambda>child. is_aligned (Min cover_ids) (obj_bits_cdl (object_type (the (cdl_objects spec child))) (object_size_bits (the (cdl_objects spec child))))) children \<Longrightarrow>
-     list_all (\<lambda>child. cdl_objects spec child \<noteq> None \<and>
-                       object_type (the (cdl_objects spec child)) \<noteq> UntypedType \<and>
-                       object_size_bits (the (cdl_objects spec child)) < 2 ^ word_bits \<and>
-                       Min cover_ids \<le> (Min cover_ids) + 2 ^ obj_bits_cdl (object_type (the (cdl_objects spec child))) (object_size_bits (the (cdl_objects spec child))) \<and>
-                       obj_bits_cdl (object_type (the (cdl_objects spec child))) (object_size_bits (the (cdl_objects spec child))) < word_size) children \<Longrightarrow>
+    "\<lbrakk> \<forall>x \<in> set children. t x = (aligned_allocations spec (Min cover_ids) children) x;
+       cover_ids \<noteq> {};
+       finite cover_ids;
+       distinct children;
+       \<forall>obj\<in>ran (cdl_objects spec). object_domain obj = minBound;
+       list_all (\<lambda>child. the (allocate (Min cover_ids) spec children child) \<in> cover_ids ) children;
+       list_all (\<lambda>child. si_caps child \<noteq> None \<and> the (si_caps child) < 2 ^ si_cnode_size) children;
+       list_all (\<lambda>child. is_aligned (Min cover_ids) (the_tbits child)) children;
+       list_all (\<lambda>child. cdl_objects spec child \<noteq> None \<and>
+                         object_type (the_obj child) \<noteq> UntypedType \<and>
+                         the_obits child < 2 ^ word_bits \<and>
+                         Min cover_ids \<le> Min cover_ids + 2 ^ the_tbits child \<and>
+                         the_tbits child < word_size) children \<rbrakk> \<Longrightarrow>
      \<lbrace>\<guillemotleft>(si_null_caps_at t si_caps spec  (set children) \<and>*
        (si_cnode_id, unat parent_cptr) \<mapsto>c UntypedCap dev cover_ids cover_ids \<and>*
        sep_map_set_conj (\<lambda>child. (the (t child)) \<mapsto>o Untyped) (set children) \<and>*
@@ -455,23 +474,31 @@ lemma create_children_wp:
       K (parent_cptr' = parent_cptr \<and> parent_cptr < 2 ^ si_cnode_size)\<rbrace>
      mapM_x (create_object spec si_caps parent_cptr) children
      \<lbrace>\<lambda>s. \<guillemotleft>(si_caps_at t si_caps spec dev (set children) \<and>*
-           (EXS remaining_ids. (si_cnode_id, unat parent_cptr') \<mapsto>c UntypedCap dev cover_ids remaining_ids) \<and>*
+           (EXS remaining_ids. (si_cnode_id, unat parent_cptr') \<mapsto>c
+                                 UntypedCap dev cover_ids remaining_ids) \<and>*
            objects_empty spec t (set children) \<and>*
            si_objects \<and>* R )\<guillemotright>\<rbrace>"
   supply Ball_set[symmetric, simp]
   apply (rule hoare_gen_asm)
   apply (case_tac children)
-   apply clarsimp
-   apply (clarsimp simp: mapM_x_def sequence_x_def, wp, clarsimp simp: si_caps_at_def si_null_caps_at_def objects_empty_def, fastforce)
+   apply (wpsimp simp: si_caps_at_def si_null_caps_at_def objects_empty_def mapM_x_def
+                       sequence_x_def)
+   apply fastforce
+  apply (rename_tac p children')
   apply (simp add: mapM_x_Cons, wp)
-    apply (rule sep_hoare_fold_mapM_x_inv[OF create_object_rest[where t="(aligned_allocations spec (Min cover_ids) children)" and base_ptr="Min cover_ids" and cover_ids = cover_ids and
-                                                                      available_ids = "cover_ids - {..<the (allocate (Min cover_ids) spec children child )}" and
-                                                                      default_child = "default_object_in spec child" and
-                                                                      child_obj = "the (cdl_objects spec child)" for list child, simplified sep_wp_simp]])
-
-  using Some_to_the apply fastforce
+    apply (rule sep_hoare_fold_mapM_x_inv[OF
+                  create_object_rest[where
+                    t = "aligned_allocations spec (Min cover_ids) children" and
+                    base_ptr = "Min cover_ids" and
+                    cover_ids = cover_ids and
+                    available_ids = "cover_ids -
+                                     {..<the (allocate (Min cover_ids) spec children child )}" and
+                    default_child = "default_object_in spec child" and
+                    child_obj = "the (cdl_objects spec child)" for list child,
+                    simplified sep_wp_simp]])
+                 apply (fastforce dest: Some_to_the)
                 apply (fastforce simp: default_object_some_default)
-  using Some_to_the apply (fastforce)
+               apply (fastforce dest: Some_to_the)
               apply fastforce
              apply fastforce
             apply fastforce
@@ -487,11 +514,16 @@ lemma create_children_wp:
      apply (subst Min_diff_upt; clarsimp?)
     apply clarsimp
    apply clarsimp
+   apply (rename_tac cap cdl_obj)
    apply (rule hoare_vcg_conj_lift)
-    apply (rule create_object_first[where base_ptr ="Min cover_ids" and cover_ids=cover_ids and obj_size = " obj_bits_cdl (object_type obj) (object_size_bits obj)" and
-                     default_child = "default_object_in spec child" for obj child, simplified sep_wp_simp, THEN sep_lift_generic])
+    apply (rule create_object_first[where
+                  base_ptr = "Min cover_ids" and
+                  cover_ids = cover_ids and
+                  obj_size = "obj_bits_cdl (object_type obj) (object_size_bits obj)" and
+                  default_child = "default_object_in spec child" for obj child,
+                  simplified sep_wp_simp, THEN sep_lift_generic])
                  apply fastforce
-  using default_object_some_default apply (fastforce)
+                apply (fastforce dest: default_object_some_default)
                apply fastforce
               apply fastforce
              apply fastforce
@@ -504,26 +536,18 @@ lemma create_children_wp:
       apply fastforce
      apply fastforce
     apply fastforce
-   apply (rule create_object_has_children[where t="(aligned_allocations spec (Min cover_ids) children)" and
-                    base_ptr ="Min cover_ids" and cover_ids=cover_ids])
-                 apply fastforce
-                apply (erule default_object_some_default)
-               apply fastforce
-              apply fastforce
+   apply (rule create_object_has_children[where
+                 t = "aligned_allocations spec (Min cover_ids) children" and
+                 base_ptr = "Min cover_ids" and
+                 cover_ids = cover_ids];
+          (solves clarsimp)?)
              apply fastforce
-            apply fastforce
-           apply fastforce
-          apply fastforce
-         apply fastforce
-        apply clarsimp
-        apply (subst aligned_allocations_hd)
-        apply (clarsimp simp: spec_object_size_def)
-       apply clarsimp
-      apply fastforce
-     apply fastforce
-    apply fastforce
-   apply fastforce
+            apply (erule default_object_some_default)
+           apply (fastforce+)[5]
+      apply (fastforce simp: spec_object_size_def aligned_allocations_hd)
+     apply (fastforce+)[3]
   apply (clarsimp simp: si_null_caps_at_def)
+  apply (rename_tac cap cdl_obj)
   apply (intro conjI)
    apply (sep_flatten, sep_cancel)
    apply (subst (asm) si_null_cap_at_cong)
@@ -550,11 +574,11 @@ lemma create_children_wp:
        apply (erule distinct_previous_const[rotated], clarsimp)
       apply clarsimp
       apply (rule_tac f="\<lambda>x. cover_ids - {..<x}" in arg_cong)
-      apply (clarsimp simp: aligned_allocations_def next_allocation_def spec_object_size_def Let_unfold)
+      apply (clarsimp simp: aligned_allocations_def next_allocation_def spec_object_size_def Let_def)
       apply (subst mapp_app)
        defer
        apply clarsimp
-      apply (case_tac list; simp)
+      apply (case_tac children'; simp)
        apply (clarsimp simp: sep_fold_def)
        apply sep_cancel
        apply (clarsimp simp: si_cap_at_def si_caps_at_def allocate_alignUp)
@@ -567,44 +591,52 @@ lemma create_children_wp:
         apply (fastforce simp: ran_def)
        apply (clarsimp simp: mapp_def)
       apply (intro conjI impI; clarsimp)
-       apply (clarsimp simp: aligned_allocate_previous allocate_previous next_allocation_def spec_object_size_def)
+       apply (rename_tac cdl_obj')
+       apply (clarsimp simp: aligned_allocate_previous allocate_previous next_allocation_def
+                            spec_object_size_def)
        apply (subst alignUp_idem, assumption, simp add: word_size_def)
        apply sep_cancel
-       apply (clarsimp simp:  sep_fold_def)
+       apply (clarsimp simp: sep_fold_def)
        apply sep_flatten
-       apply (sep_erule si_null_cap_at_cong[THEN extD1, rotated])
+       apply (sep_erule si_null_cap_at_cong[THEN fun_congD1, rotated])
         apply (erule trans)
         apply (clarsimp simp: alignUp_idem word_size_def)
-        apply (simp add: aligned_allocate_previous next_allocation_def spec_object_size_def alignUp_idem word_size_def)
+        apply (simp add: aligned_allocate_previous next_allocation_def spec_object_size_def
+                         alignUp_idem word_size_def)
        apply (clarsimp simp: alignUp_idem word_size_def)
-       apply (simp add: aligned_allocate_previous next_allocation_def spec_object_size_def alignUp_idem word_size_def)
+       apply (simp add: aligned_allocate_previous next_allocation_def spec_object_size_def
+                        alignUp_idem word_size_def)
        apply sep_cancel+
        apply (clarsimp simp: si_caps_at_def)
-       apply (sep_flatten, sep_erule si_cap_at_cong[THEN extD1, rotated])
+       apply (sep_flatten, sep_erule si_cap_at_cong[THEN fun_congD1, rotated])
         apply (erule trans[symmetric])
         apply (simp add: aligned_allocations_def)
         apply (subst alignUp_idem, assumption, simp add: word_size_def, rule refl)
-       apply (sep_erule si_cap_at_cong[THEN extD1, rotated])
+       apply (sep_erule si_cap_at_cong[THEN fun_congD1, rotated])
         apply (erule trans[symmetric])
         apply (simp add: aligned_allocations_def)
         apply (subst mapp_app; clarsimp)
          apply (clarsimp simp: allocate.simps)
-        apply (simp add: allocate.simps aligned_allocate_previous next_allocation_def spec_object_size_def alignUp_idem word_size_def Let_unfold)
-       apply (rule exI, sep_cancel+)
+        apply (simp add: allocate.simps aligned_allocate_previous next_allocation_def
+                         spec_object_size_def alignUp_idem word_size_def Let_unfold)
+       apply (rule exI, sep_cancel)
        apply (clarsimp simp: objects_empty_def object_empty_def object_initialised_general_def)
-       apply (simp add: aligned_allocate_previous next_allocation_def spec_object_size_def alignUp_idem word_size_def Let_unfold default_object_in_def object_default_state_def)
-       apply (frule_tac x=ya in bspec)
+       apply (simp add: aligned_allocate_previous next_allocation_def spec_object_size_def
+                        alignUp_idem word_size_def Let_unfold default_object_in_def
+                        object_default_state_def)
+       apply (frule_tac x=cdl_obj in bspec)
         apply (fastforce simp: ran_def, clarsimp)
-       apply (frule_tac x=yc in bspec)
+       apply (frule_tac x=cdl_obj' in bspec)
         apply (fastforce simp: ran_def, clarsimp)
        apply sep_solve
       apply (simp add: allocate_previous spec_object_size_def Let_unfold)
       apply (simp add: next_allocation_def alignUp_idem word_size_def spec_object_size_def Let_unfold)
       apply sep_cancel
       apply (rule sep_map_sep_foldI, clarsimp, sep_flatten)
-      apply (simp add: aligned_allocate_previous allocate_previous alignUp_idem word_size_def next_allocation_def spec_object_size_def  Let_unfold)
+      apply (simp add: aligned_allocate_previous allocate_previous alignUp_idem word_size_def
+                       next_allocation_def spec_object_size_def  Let_unfold)
       apply sep_cancel
-      apply (clarsimp simp: sep_list_conj_map_add sep_list_conj_sep_map_set_conj)
+      apply (clarsimp simp: sep_list_conj_sep_map_set_conj)
       apply (subst sep_map_set_conj_subst[OF arg_cong[where f="\<lambda>p. p \<mapsto>o Untyped"]])
        apply (subst aligned_allocate_previous, simp, simp)
         apply (rule option.collapse)
@@ -619,238 +651,245 @@ lemma create_children_wp:
       apply (simp only: option.sel)
       apply sep_cancel
       apply (clarsimp simp: si_caps_at_def)
-      apply (sep_erule si_null_cap_at_cong[THEN extD1, rotated])
+      apply (sep_erule si_null_cap_at_cong[THEN fun_congD1, rotated])
        apply (erule trans)
-       apply (simp add: aligned_allocations_def aligned_allocate_previous alignUp_idem word_size_def next_allocation_def spec_object_size_def Let_unfold)
+       apply (simp add: aligned_allocations_def aligned_allocate_previous alignUp_idem word_size_def
+                        next_allocation_def spec_object_size_def Let_unfold)
        apply (subst mapp_app; clarsimp)
         apply (clarsimp simp: allocate.simps)
-       apply (simp add: allocate.simps aligned_allocate_previous next_allocation_def spec_object_size_def alignUp_idem word_size_def Let_unfold)
-      apply (sep_erule sep_map_set_conj_subst[THEN extD1, OF si_null_cap_at_cong, rotated ])
+       apply (simp add: allocate.simps aligned_allocate_previous next_allocation_def
+                        spec_object_size_def alignUp_idem word_size_def Let_unfold)
+      apply (sep_erule sep_map_set_conj_subst[THEN fun_congD1, OF si_null_cap_at_cong, rotated])
        apply (drule (1) bspec, erule trans)
        apply (rule allocate_alignUp[symmetric]; clarsimp?)
       apply sep_cancel+
-      apply (sep_erule si_cap_at_cong[THEN extD1, rotated])
-       apply (simp add: aligned_allocate_previous alignUp_idem word_size_def next_allocation_def spec_object_size_def Let_unfold)
-      apply (sep_erule si_cap_at_cong[THEN extD1, rotated])
+      apply (sep_erule si_cap_at_cong[THEN fun_congD1, rotated])
+       apply (simp add: aligned_allocate_previous alignUp_idem word_size_def next_allocation_def
+                        spec_object_size_def Let_unfold)
+      apply (sep_erule si_cap_at_cong[THEN fun_congD1, rotated])
        apply (erule trans[symmetric])
-       apply (simp add: aligned_allocate_previous alignUp_idem word_size_def next_allocation_def spec_object_size_def Let_unfold)
-      apply (sep_erule sep_map_set_conj_subst[THEN extD1, OF si_cap_at_cong, rotated ])
+       apply (simp add: aligned_allocate_previous alignUp_idem word_size_def next_allocation_def
+                        spec_object_size_def Let_unfold)
+      apply (sep_erule sep_map_set_conj_subst[THEN fun_congD1, OF si_cap_at_cong, rotated ])
        apply (drule (1) bspec, erule trans[symmetric])
-       apply (simp add: aligned_allocate_previous alignUp_idem word_size_def next_allocation_def spec_object_size_def Let_unfold)
+       apply (simp add: aligned_allocate_previous alignUp_idem word_size_def next_allocation_def
+                        spec_object_size_def Let_unfold)
        apply (rule allocate_alignUp[symmetric]; clarsimp?)
       apply (rule exI, sep_cancel+)
       apply (clarsimp simp: objects_empty_def)
       apply (sep_erule default_object_is_object_empty)
          apply fastforce
         apply (fastforce simp: ran_def)
-       apply (simp add:aligned_allocations_def aligned_allocate_previous alignUp_idem word_size_def next_allocation_def spec_object_size_def Let_unfold)
+       apply (simp add: aligned_allocations_def aligned_allocate_previous alignUp_idem word_size_def
+                        next_allocation_def spec_object_size_def Let_unfold)
       apply (sep_erule default_object_is_object_empty)
          apply fastforce
-        apply (fastforce simp: ran_def)
+        subgoal by (fastforce simp: ran_def) (* slow *)
        apply (simp add: aligned_allocations_def)
       apply (subst (asm) sep_map_set_conj_subst[OF arg_cong[where f="\<lambda>p. p \<mapsto>o val" for val]])
+      apply (rename_tac x)
        apply (rule arg_cong[where f=the and y="t _"])
        apply (drule (1) bspec, rule sym, erule trans, rule allocate_alignUp[symmetric])
         apply clarsimp
        apply clarsimp
       apply (erule sep_map_set_elim, rule refl)
-      apply (drule_tac x=x in bspec, assumption, elim conjE exE, erule (1) default_object_is_object_empty)
+      apply (drule_tac x=x in bspec, assumption, elim conjE exE,
+             erule (1) default_object_is_object_empty)
        apply (fastforce simp: ran_def)
       apply fastforce
      apply sep_cancel
      apply sep_cancel
      apply sep_cancel
-     apply (sep_erule si_null_cap_at_cong[THEN extD1, rotated])
+     apply (sep_erule si_null_cap_at_cong[THEN fun_congD1, rotated])
       apply assumption
      apply (rule TrueI)
     apply (subst aligned_allocations_def)
     apply clarsimp
+    apply (rename_tac prev p')
     apply (subst mapp_app)
      apply clarsimp
      apply (erule previous_in_allocate; clarsimp)
     apply clarsimp
     apply (subst unat_gt_0)
-    apply (rule sub_neq_zero_le)
-    apply (subgoal_tac "alignUp (the (allocate (Min cover_ids) spec (a # list) x)) (spec_object_size spec x) +
-                2 ^ obj_bits_cdl (object_type (the (cdl_objects spec x))) (object_size_bits (the (cdl_objects spec x))) = next_allocation spec (the (allocate (Min cover_ids) spec (a # list)  x)) x ")
+    apply (rule word_sub_neq_zero_le)
+    apply (subgoal_tac "alignUp (the (allocate (Min cover_ids) spec (p # children') prev))
+                                (spec_object_size spec prev) +
+                        2 ^ obj_bits_cdl (object_type (the (cdl_objects spec prev)))
+                                         (object_size_bits (the (cdl_objects spec prev)))
+                        = next_allocation spec
+                                          (the (allocate (Min cover_ids) spec (p # children') prev))
+                                          prev")
      apply simp
      apply (subst allocate_previous[THEN Some_the, symmetric]; simp?)
-       defer
-  using distinct_previous_const apply fastforce
-      apply (rule_tac x=yb in increasing_allocations[simplified, THEN ballE])
-       apply (clarsimp simp: in_tail_previous)
-      apply fastforce
-     apply (clarsimp simp: next_allocation_def spec_object_size_def Let_unfold)
-    apply clarsimp
-    apply (rule_tac x=x in aligned_no_wrap[simplified, THEN ballE])
-     apply (clarsimp simp: next_allocation_def spec_object_size_def Let_unfold)
-    apply (simp add: previous_in_list)
+       prefer 2
+       apply (fastforce dest!: distinct_previous_const[rotated])
+      apply blast
+     apply (rule_tac x=p' in increasing_allocations[simplified, THEN ballE])
+      apply (clarsimp simp: in_tail_previous)
+     apply fastforce
+    apply (clarsimp simp: next_allocation_def spec_object_size_def Let_unfold)
    apply clarsimp
-   apply (meson distinct.simps(2) previous_in_allocate)
-  apply blast
+   apply (rename_tac prev p')
+   apply (rule_tac x=prev in aligned_no_wrap[simplified, THEN ballE])
+    apply (clarsimp simp: next_allocation_def spec_object_size_def Let_unfold)
+   apply (simp add: previous_in_list)
+  apply clarsimp
+  apply (meson distinct.simps(2) previous_in_allocate)
   done
 
-lemma untyped_cap_helper: "is_device_cap ut =  dev \<Longrightarrow> is_full_untyped_cap ut \<Longrightarrow> UntypedCap dev (available_range ut) (available_range ut) = ut"
-  by (clarsimp simp:  is_full_untyped_cap_def dev_of_def split: cdl_cap.splits)
+lemma untyped_cap_helper:
+  "\<lbrakk> is_device_cap ut = dev; is_full_untyped_cap ut \<rbrakk> \<Longrightarrow>
+   UntypedCap dev (available_range ut) (available_range ut) = ut"
+  by (clarsimp simp: is_full_untyped_cap_def dev_of_def split: cdl_cap.splits)
 
-definition derivation_set :: "('a \<times> ('b list)) list \<Rightarrow> ('a \<times> 'b) set"
-   where "derivation_set xs = set (List.bind xs (\<lambda>(parent,children). List.bind children (swp (#) [] o Pair parent)))"
+definition derivation_set :: "('a \<times> ('b list)) list \<Rightarrow> ('a \<times> 'b) set" where
+  "derivation_set xs \<equiv>
+     set (List.bind xs (\<lambda>(parent, children). List.bind children (swp (#) [] \<circ> Pair parent)))"
 
-lemma distinct_map_snd: "distinct_sets (map (set \<circ> snd) untyped_derivations) \<Longrightarrow> \<forall>(x,y)\<in>set untyped_derivations. \<forall>(a,b)\<in>set untyped_derivations. set b \<inter> set y \<noteq> {} \<longrightarrow> a = x"
-  apply (clarsimp)
+lemma distinct_map_snd:
+  "distinct_sets (map (set \<circ> snd) untyped_derivations) \<Longrightarrow>
+   \<forall>(x,y)\<in>set untyped_derivations. \<forall>(a,b)\<in>set untyped_derivations. set b \<inter> set y \<noteq> {} \<longrightarrow> a = x"
+  apply clarsimp
   apply (induct untyped_derivations; clarsimp simp: comp_def split: prod.splits)
-  apply (safe; clarsimp)
-  apply (subgoal_tac "x \<in> set b \<inter> (\<Union>x\<in>set untyped_derivations. set (snd x))")
-  apply (clarsimp)
-  apply fastforce
- apply (subgoal_tac "x \<in> set b \<inter> (\<Union>x\<in>set untyped_derivations. set (snd x))")
-  apply (clarsimp)
-  apply fastforce
-  apply (atomize)
-  apply (clarsimp)
-  apply (erule_tac x="aaa" in allE)
-  apply (erule_tac x="baa" in allE)
-  apply (clarsimp)
-  apply (fastforce)
-done
+  apply (metis (lifting) Union_disjoint image_eqI inf_commute snd_conv)
+  done
 
+lemma is_in_rangeD:
+  "\<lbrakk> ((=) s' \<and>* R) s; v \<in> dom s' \<rbrakk> \<Longrightarrow> s v = s' v"
+  by (clarsimp simp: sep_conj_def plus_fun_def plus_option_def)
 
-abbreviation (input) "is \<equiv> (=)"
+lemma is_in_sep_list_conjD:
+  "\<lbrakk> sep_list_conj (map (\<lambda>x. (=) (s' x)) xs) s; x \<in> set xs; v \<in> dom (s' x) \<rbrakk> \<Longrightarrow>
+   s v = (s' x v :: 'b option)"
+  apply (subst (asm) sep_list_conj_map_remove1, assumption)
+  apply (erule (1) is_in_rangeD)
+  done
 
-lemma is_in_rangeD: "(is g \<and>* R) s \<Longrightarrow> v \<in> dom g \<Longrightarrow> s v = g v"
-  apply (clarsimp simp: sep_conj_def)
-  apply (clarsimp simp: plus_fun_def plus_option_def)
-done
+definition disjoint_sets :: "'a set set \<Rightarrow> bool" where
+  "disjoint_sets S \<equiv> \<forall>x\<in>S. \<forall>y\<in>S. x \<noteq> y \<longrightarrow> x \<inter> y = {}"
 
-lemma is_in_sep_list_conjD: "sep_list_conj (map (\<lambda>x. is (g x)) xs) s \<Longrightarrow>  x \<in> set xs \<Longrightarrow>  v \<in> dom (g x) \<Longrightarrow> s v = (g x v :: 'b option) "
-    apply (subst (asm) sep_list_conj_map_remove1, assumption)
-    apply (erule (1) is_in_rangeD)
-done
+lemma distinct_disjoint:
+  "distinct_sets xs \<Longrightarrow> disjoint_sets (set xs)"
+  by (induct xs)
+     (auto simp: disjoint_sets_def)
 
-definition "disjoint_sets S \<equiv> \<forall>x\<in>S. \<forall>y\<in>S. x \<noteq> y \<longrightarrow> x \<inter> y = {}"
-
-
-lemma distinct_disjoint: "distinct_sets S \<Longrightarrow> disjoint_sets (set S)"
-  apply (induct S; clarsimp simp: disjoint_sets_def)
-  by (intro conjI ballI impI; blast)
-
-
-lemma helper: "distinct_sets (map (set \<circ> snd) untyped_derivations)
-         \<Longrightarrow> \<forall>s s'. s \<in> (\<lambda>x. set (snd x)) ` set untyped_derivations \<and> s' \<in> (\<lambda>x. set (snd x)) ` set untyped_derivations \<longrightarrow> s \<noteq> s' \<longrightarrow> s \<inter> s' = {}"
+lemma distinct_sets_helper:
+  "distinct_sets (map (set \<circ> snd) untyped_derivations) \<Longrightarrow>
+   \<forall>s s'. s \<in> (\<lambda>x. set (snd x)) ` set untyped_derivations \<and>
+          s' \<in> (\<lambda>x. set (snd x)) ` set untyped_derivations \<longrightarrow> s \<noteq> s' \<longrightarrow> s \<inter> s' = {}"
   apply (drule distinct_disjoint)
-  apply (clarsimp simp: comp_def)
-   apply (clarsimp simp: disjoint_sets_def)
-  by (metis snd_conv)
+  apply (clarsimp simp: comp_def disjoint_sets_def)
+  apply (metis snd_conv)
+  done
 
-lemma [simp]: "unat x = unat y \<longleftrightarrow> x = y"
-  by (metis not_less order_antisym_conv order_refl unat_mono)
+lemma zip_map_eq_map:
+  "(zip (map f xs) ys) = map (apfst f) (zip xs ys)"
+  apply (induct xs arbitrary: ys ; clarsimp)
+  apply (clarsimp simp: apfst_def)
+  apply (metis id_apply list.map_id0 list.simps(9) map_prod_def zip_map_map)
+  done
 
-lemma zip_map_map: "(zip (map f xs) ys) = map (apfst f) (zip xs ys)"
- apply (induct xs arbitrary: ys ; clarsimp)
- apply (clarsimp simp: apfst_def)
-  by (metis id_apply list.map_id0 list.simps(9) map_prod_def zip_map_map)
+definition on_depleted_untyped_cap  :: "(cdl_cap \<Rightarrow> 'a \<Rightarrow> bool) \<Rightarrow> cdl_cap \<Rightarrow> 'a \<Rightarrow> bool" where
+  "on_depleted_untyped_cap P \<equiv>
+     \<lambda>cap s. \<exists>cap'. is_untyped_cap cap \<and>
+                    is_device_cap cap = is_device_cap cap' \<and>
+                    untyped_cap_range cap = untyped_cap_range cap' \<and>
+                    P cap' s"
 
+lemma distinct_fst_snd_distinct:
+  "\<lbrakk> distinct_sets (map (set \<circ> snd) xs);  distinct (map fst xs) \<rbrakk> \<Longrightarrow> distinct xs"
+  apply (induct xs; clarsimp simp: comp_def)
+  apply (fastforce simp: Int_commute Union_disjoint image_def)
+  done
 
-
-lemma prod_lift_lambda: "(\<lambda>x. f (case x of (a,b) \<Rightarrow> g a b)) = (\<lambda>(a,b). f (g a b)) "
- by (rule ext, clarsimp)
-
-
-definition
- on_depleted_untyped_cap where
-  "on_depleted_untyped_cap P \<equiv> (\<lambda>cap s. \<exists>cap'. is_untyped_cap cap \<and> is_device_cap cap = is_device_cap cap' \<and> untyped_cap_range cap = untyped_cap_range cap' \<and> P cap' s)"
-
-lemma distinct_fst_snd_distinct: "distinct_sets (map (set o snd) S) \<Longrightarrow>  distinct (map fst S) \<Longrightarrow>  distinct S "
-  apply (induct S; clarsimp simp: comp_def)
-  apply (subst (asm) Int_commute, simp add: Union_disjoint image_def)
- by (fastforce)
-
-lemma child_in_collection[simp]:
-       "(a, b) \<in> set untyped_derivations \<Longrightarrow> child \<in> set b
-       \<Longrightarrow> child \<in> set (collect_children untyped_derivations)"
+lemma child_in_collection:
+  "\<lbrakk> (a, b) \<in> set untyped_derivations; child \<in> set b \<rbrakk> \<Longrightarrow>
+   child \<in> set (collect_children untyped_derivations)"
   by (fastforce simp: collect_children_def List.bind_def Bex_def)
 
+lemma the_map_of_elim:
+  "\<lbrakk> x \<in> set xs; length xs \<le> length ys; \<forall>x\<in>set ys. P x \<rbrakk> \<Longrightarrow> P (the (map_of (zip xs ys) x))"
+  apply (induct xs arbitrary: ys; clarsimp)
+  apply (rename_tac ys, case_tac ys; clarsimp)
+  done
 
-lemma the_map_of_elim[simp, elim]: "x \<in> set xs \<Longrightarrow> length xs \<le> length ys \<Longrightarrow> \<forall>x\<in>set ys. P x \<Longrightarrow> P (the (map_of (zip xs ys) x))"
-     apply (induct xs arbitrary: ys; clarsimp)
-     by (case_tac ys; clarsimp)
-
-
-
-lemma distinct_map_comp:" distinct (map g xs) \<Longrightarrow> inj f  \<Longrightarrow> distinct (map (\<lambda>a. f (g a)) xs)"
+lemma distinct_map_comp:
+  "\<lbrakk> distinct (map g xs); inj f \<rbrakk> \<Longrightarrow> distinct (map (\<lambda>a. f (g a)) xs)"
   by (meson List.distinct_map injD inj_on_def)
 
-lemma distinct_map_comp':" distinct (map g xs) \<Longrightarrow> inj f  \<Longrightarrow> distinct (map (f o g) xs)"
-  by (clarsimp simp:  comp_def distinct_map_comp)
+lemma distinct_map_comp':
+  "\<lbrakk> distinct (map g xs); inj f \<rbrakk> \<Longrightarrow> distinct (map (f o g) xs)"
+  by (clarsimp simp: comp_def distinct_map_comp)
 
-
-lemma map_allocates[simp]: "(parent, children) \<in> set untyped_derivations \<Longrightarrow> child \<in> set children \<Longrightarrow>
-                       sep_list_conj (map (\<lambda>(parent, children). is (aligned_allocations spec (f parent)  children)) untyped_derivations) t \<Longrightarrow>
-                       t child =  aligned_allocations spec (f parent) children child "
+lemma map_allocates:
+  "\<lbrakk> (parent, children) \<in> set utds; child \<in> set children;
+     (\<And>* (map (\<lambda>(p, c). (=) (aligned_allocations spec (f p) c)) utds)) s \<rbrakk>
+   \<Longrightarrow> s child = aligned_allocations spec (f parent) children child"
   apply (subst (asm) split_beta')
-  apply (drule_tac is_in_sep_list_conjD[where x="(parent,children)" and g="\<lambda>x. (aligned_allocations spec (f (fst x)) (snd x))" and xs=untyped_derivations])
- prefer 3
-  apply (erule trans)
-  apply (clarsimp)+
-  apply (clarsimp simp: aligned_allocations_def mapp_def)
-  by (simp add: in_list_allocate)
+  apply (drule_tac is_in_sep_list_conjD[where x = "(parent, children)"
+                                          and s' = "\<lambda>x. aligned_allocations spec (f (fst x)) (snd x)"
+                                          and xs = utds], assumption)
+   prefer 2
+   apply (fastforce elim: trans)
+  apply (clarsimp simp: aligned_allocations_def mapp_def in_list_allocate)
+  done
 
-lemma full_cap_range_available[elim]: "is_full_untyped_cap b \<Longrightarrow> untyped_cap_range b = available_range b"
+lemma full_cap_range_available[elim!]:
+  "is_full_untyped_cap b \<Longrightarrow> untyped_cap_range b = available_range b"
   by (cases b; clarsimp simp: is_full_untyped_cap_def)
 
+lemma untyped_derivations_inject:
+  "\<lbrakk> distinct_sets (map (set \<circ> snd) utds); list_all distinct (map snd utds) \<rbrakk> \<Longrightarrow>
+   \<forall>x y. x \<in> set utds \<longrightarrow> y \<in> set utds \<longrightarrow> x \<noteq> y \<longrightarrow> set (snd x) = set (snd y) \<longrightarrow> set (snd x) = {}"
+  apply (induct utds; clarsimp)
+  apply (metis (no_types, lifting) Int_commute Union_disjoint inf_idem rev_image_eqI set_empty
+                                   snd_conv)
+  done
 
-lemma untyped_derivations_inject[simp]: "distinct_sets (map (set o snd) untyped_derivations) \<Longrightarrow> list_all distinct (map snd untyped_derivations) \<Longrightarrow>
-    \<forall>x y. x \<in> set untyped_derivations \<longrightarrow> y \<in> set untyped_derivations \<longrightarrow> x \<noteq> y \<longrightarrow> set (snd x) = set (snd y) \<longrightarrow> set (snd x) = {}"
-   apply (clarsimp)
-   apply (induct untyped_derivations; clarsimp)
-   by (metis (no_types, lifting) Int_commute Union_disjoint inf_idem rev_image_eqI set_empty snd_conv)
+lemma distinct_inj_on:
+  "distinct (map f xs) \<Longrightarrow> inj_on f (set xs)"
+  by (induct xs; clarsimp)
 
-lemma distinct_inj_on: "distinct (map f S) \<Longrightarrow> inj_on f (set S)"
- apply (induct S; clarsimp)
-done
-
-definition "dupl x = (x,x)"
-
-lemma [simp]: "sep_map_set_conj (\<lambda>y. (EXS x. P x y \<and>* Q y)) S = (sep_map_set_conj (\<lambda>y. (EXS x. P x y)) S \<and>* sep_map_set_conj Q S)"
+lemma set_sep_conj_ex_dist[simp]: (* FIXME: move to SepAlgebra; update SETSEPCONJ syntax to new form *)
+  "(SETSEPCONJ y:S. (EXS x. P x y \<and>* Q y)) =
+   ((SETSEPCONJ y:S. (EXS x. P x y)) \<and>* sep_map_set_conj Q S)"
   by (subst sep.prod.cong[OF refl, OF sep_conj_exists1[symmetric]], simp only: sep.prod.distrib)
 
+lemma sep_map_set_conj_fold_fst:
+  "(sep_map_set_conj (\<lambda>x. P (fst x)) S) = sep_map_set_conj ((\<lambda>x. P x) \<circ> fst) S"
+  by simp
 
-method arg_checker for t = (match conclusion in "x = _" for x \<Rightarrow> \<open>match (x) in t \<Rightarrow> \<open>fail\<close> \<bar> _ \<Rightarrow> \<open>rule refl\<close> \<close>)
-
-method comp_folder uses comp = ( (subst comp, arg_checker "(\<lambda>a. a)", arg_checker "(\<lambda>a. a)") |  (subst (asm) comp, arg_checker "(\<lambda>a. a)", arg_checker "(\<lambda>a. a)"))
-
-lemma comp_folder: "f = f \<Longrightarrow> g = g \<Longrightarrow> (\<lambda>x. f (g x)) = f o g " by (clarsimp simp: comp_def)
-
-lemma distinct_fstD:
+lemma distinct_fstD: (* FIXME: move to Lib *)
   "distinct (map fst xs) \<Longrightarrow> distinct xs"
   by (induct xs; fastforce simp: image_def)
 
 lemma the_map_of_zip_inR:
-  "x \<in> set xs \<Longrightarrow> length xs \<le> length ys \<Longrightarrow> the (map_of (zip xs ys) x) \<in> set ys"
+  "\<lbrakk> x \<in> set xs; length xs \<le> length ys \<rbrakk> \<Longrightarrow> the (map_of (zip xs ys) x) \<in> set ys"
   apply (induct xs arbitrary: ys; clarsimp)
-  by (case_tac ys; clarsimp)
+  apply (rename_tac ys, case_tac ys; clarsimp)
+  done
 
 definition matching_paddrs where
   "matching_paddrs ut_ids ut_info \<equiv>
-    (\<forall>id \<in> set ut_ids. \<exists>desc. desc \<in> set ut_info \<and> bi_ut_paddr desc = id)"
+     \<forall>id \<in> set ut_ids. \<exists>desc. desc \<in> set ut_info \<and> bi_ut_paddr desc = id"
 
 definition valid_untypeds where
   "valid_untypeds ut_ids ut_cptrs ut_info ut_caps \<equiv>
-    length ut_ids = length ut_cptrs \<and>
-    length ut_cptrs = length ut_info \<and>
-    length ut_cptrs = length ut_caps \<and>
-    distinct (map bi_ut_paddr ut_info) \<and>
-    matching_paddrs ut_ids ut_info \<and>
-    distinct ut_cptrs \<and>
-    distinct_sets (map cap_free_ids ut_caps) \<and>
-    list_all is_full_untyped_cap ut_caps \<and>
-    list_all (\<lambda>cap. available_range cap \<noteq> {}) ut_caps \<and>
-    list_all well_formed_untyped_cap ut_caps \<and>
-    list_all (\<lambda>c. \<not> is_device_cap c) ut_caps"
+     length ut_ids = length ut_cptrs \<and>
+     length ut_cptrs = length ut_info \<and>
+     length ut_cptrs = length ut_caps \<and>
+     distinct (map bi_ut_paddr ut_info) \<and>
+     matching_paddrs ut_ids ut_info \<and>
+     distinct ut_cptrs \<and>
+     distinct_sets (map cap_free_ids ut_caps) \<and>
+     list_all is_full_untyped_cap ut_caps \<and>
+     list_all (\<lambda>cap. available_range cap \<noteq> {}) ut_caps \<and>
+     list_all well_formed_untyped_cap ut_caps \<and>
+     list_all (\<lambda>c. \<not> is_device_cap c) ut_caps"
 
 definition make_untyped_map ::
-  "cdl_object_id list \<Rightarrow> cdl_cptr list \<Rightarrow> bi_untyped_desc list \<Rightarrow> cdl_cap list \<Rightarrow>
-   cdl_object_id \<Rightarrow> (cdl_cptr \<times> bi_untyped_desc \<times> cdl_cap) option"
+  "cdl_object_id list \<Rightarrow> cdl_cptr list \<Rightarrow> bi_untyped_desc list \<Rightarrow> cdl_cap list \<Rightarrow> cdl_object_id \<Rightarrow>
+   (cdl_cptr \<times> bi_untyped_desc \<times> cdl_cap) option"
   where
   "make_untyped_map untyped_ids untyped_cptrs untyped_info untyped_caps \<equiv> \<lambda>untyped_id.
      if untyped_id \<in> set untyped_ids
@@ -864,13 +903,13 @@ lemma make_untyped_map_Some:
     length cptrs = length caps\<rbrakk> \<Longrightarrow>
    \<exists>n. (make_untyped_map ids cptrs info caps ut_id) = Some (cptrs ! n, info ! n, caps ! n) \<and>
        bi_ut_paddr (info ! n) = ut_id \<and> n < length ids"
-  apply (clarsimp simp: make_untyped_map_def matching_paddrs_def find_Some_iff
-         split_def)
+  apply (clarsimp simp: make_untyped_map_def matching_paddrs_def find_Some_iff split_def)
   apply (drule_tac x=ut_id in bspec; clarsimp)
   apply (clarsimp simp: in_set_conv_nth)
-  apply (rule_tac x=ia in exI)
+  apply (rename_tac i i')
+  apply (rule_tac x=i' in exI)
   apply clarsimp
-  apply (rule_tac x=ia in exI)
+  apply (rule_tac x=i' in exI)
   apply clarsimp
   apply (subst (asm) nth_map[where f=bi_ut_paddr, symmetric], clarsimp)+
   apply (subst (asm) nth_eq_iff_index_eq; clarsimp)
@@ -881,8 +920,8 @@ lemma make_untyped_map_Some':
     length ids = length cptrs; length cptrs = length info;
     length cptrs = length caps\<rbrakk> \<Longrightarrow>
    \<exists>x. (make_untyped_map ids cptrs info caps ut_id) = Some x"
-  apply (frule make_untyped_map_Some; assumption?)
-  by auto
+  using make_untyped_map_Some
+  by blast
 
 lemma cap_of_make_untyped_map:
   "\<lbrakk>ut_id \<in> set ids; matching_paddrs ids info; distinct (map bi_ut_paddr info);
@@ -912,20 +951,20 @@ lemma make_untyped_map_reorder'[OF refl, simplified]:
        = make_untyped_map ids cptrs info caps"
   apply (rule ext)
   apply (case_tac "x \<in> set ids")
-   prefer 2
-   apply (clarsimp simp: make_untyped_map_def)
-  apply (frule make_untyped_map_Some; assumption?)
-  apply (clarsimp simp: in_set_conv_nth)
-
-  apply (clarsimp simp: make_untyped_map_def o_def)
-  apply (subst find_Some_iff)
-
-  apply clarsimp
-  apply (rule_tac x=i in exI)
-  apply clarsimp
-  apply (frule_tac ut_id="ids ! j" and cptrs=cptrs and info=info and caps=caps in make_untyped_map_Some[rotated];
-         clarsimp)
-  apply (clarsimp simp: make_untyped_map_def distinct_conv_nth)
+   apply (frule make_untyped_map_Some; assumption?)
+   apply (clarsimp simp: in_set_conv_nth)
+   apply (rename_tac i n)
+   apply (clarsimp simp: make_untyped_map_def o_def)
+   apply (subst find_Some_iff)
+   apply clarsimp
+   apply (rule_tac x=i in exI)
+   apply clarsimp
+   apply (rename_tac j x a b)
+   apply (frule_tac ut_id="ids ! j" and cptrs=cptrs and info=info and caps=caps
+                    in make_untyped_map_Some[rotated];
+          clarsimp)
+   apply (clarsimp simp: make_untyped_map_def distinct_conv_nth)
+  apply (clarsimp simp: make_untyped_map_def)
   done
 
 lemma make_untyped_map_cptr_inj_on:
@@ -934,11 +973,7 @@ lemma make_untyped_map_cptr_inj_on:
     length cptrs = length caps; distinct cptrs\<rbrakk> \<Longrightarrow>
    inj_on (cptr_of \<circ> make_untyped_map ids cptrs info caps) (set ids)"
   apply (clarsimp simp: inj_on_def)
-  apply (frule_tac ut_id="x" and cptrs=cptrs and caps=caps in make_untyped_map_Some[rotated];
-       (clarsimp simp: distinct_conv_nth))
-  apply (frule_tac ut_id="y" and cptrs=cptrs and caps=caps in make_untyped_map_Some[rotated];
-       (clarsimp simp: distinct_conv_nth))
-  apply blast
+  apply (metis Some_to_the distinct_conv_nth fst_conv make_untyped_map_Some)
   done
 
 lemma make_untyped_map_list_set[OF refl, simplified]:
@@ -949,18 +984,21 @@ lemma make_untyped_map_list_set[OF refl, simplified]:
    set (zip (map fst sorted_list) (map (snd \<circ> snd) sorted_list))
    = set (zip cptrs caps)"
   apply (rule subset_antisym; clarsimp simp: in_set_zip)
-   apply (frule_tac ut_id="ids ! n" and cptrs=cptrs and info=info and caps=caps in make_untyped_map_Some[rotated];
-        (clarsimp simp: distinct_conv_nth))
+  apply (rename_tac n)
+  apply (frule_tac ut_id="ids ! n" and cptrs=cptrs and info=info and caps=caps
+                   in make_untyped_map_Some[rotated];
+         clarsimp simp: distinct_conv_nth)
    apply fastforce
-
   apply (cut_tac make_untyped_map_cptr_inj_on[where ids=ids and cptrs=cptrs and caps=caps];
          fastforce?)
   apply (subst (asm) surjective_iff_injective_gen[where T="set cptrs", symmetric];
          (clarsimp simp: distinct_card cptr_of_make_untyped_map)?)
   apply (drule_tac x="cptrs ! n" in bspec; clarsimp)
   apply (clarsimp simp: in_set_conv_nth)
-  apply (frule_tac ut_id="ids ! i" and cptrs=cptrs and info=info and caps=caps in make_untyped_map_Some[rotated];
-         (clarsimp simp: distinct_conv_nth))
+  apply (rename_tac i)
+  apply (frule_tac ut_id="ids ! i" and cptrs=cptrs and info=info and caps=caps
+                   in make_untyped_map_Some[rotated];
+         clarsimp simp: distinct_conv_nth)
   apply (rule_tac x=i in exI)
   apply fastforce
   done
@@ -971,11 +1009,15 @@ lemma make_untyped_map_distinct_fst:
     length cptrs = length caps; distinct ids; distinct cptrs\<rbrakk> \<Longrightarrow>
    distinct (map (fst \<circ> (the \<circ> make_untyped_map ids cptrs info caps)) ids)"
   apply (clarsimp simp: distinct_conv_nth)
-  apply (frule_tac ut_id="ids ! i" and cptrs=cptrs and info=info and caps=caps in make_untyped_map_Some[rotated];
-         (clarsimp simp: distinct_conv_nth))
-  apply (frule_tac ut_id="ids ! j" and cptrs=cptrs and info=info and caps=caps in make_untyped_map_Some[rotated];
-         (clarsimp simp: distinct_conv_nth))
-  apply (case_tac "n=na"; clarsimp)
+  apply (rename_tac i j)
+  apply (frule_tac ut_id="ids ! i" and cptrs=cptrs and info=info and caps=caps
+                   in make_untyped_map_Some[rotated];
+         clarsimp simp: distinct_conv_nth)
+  apply (frule_tac ut_id="ids ! j" and cptrs=cptrs and info=info and caps=caps
+                   in make_untyped_map_Some[rotated];
+         clarsimp simp: distinct_conv_nth)
+  apply (rename_tac n n')
+  apply (case_tac "n=n'"; clarsimp)
   done
 
 lemma make_untyped_map_reorder:
@@ -1008,15 +1050,10 @@ lemma sep_prod_make_untyped_map_zip[OF refl]:
    \<Longrightarrow> (SETSEPCONJ x:set ids. f (cptr_of (untyped_map x)) (cap_of (untyped_map x))) =
        (SETSEPCONJ x:set (zip cptrs caps). f (fst x) (snd x))"
   apply (cut_tac untyped_map=untyped_map in make_untyped_map_reorder, assumption+)
-  apply clarsimp
-  apply (clarsimp simp: sep_list_conj_sep_map_set_conj[symmetric] distinct_zipI1)
-
-  apply (subst map_nth_length[symmetric, where xs=ids])
-  apply (subst map_nth_length[symmetric, where xs="zip cptrs' caps'" for cptrs' caps'])
-  apply clarsimp
-
-  apply (rule map_sep_list_conj_cong)
-  apply clarsimp
+  apply (fastforce simp: sep_list_conj_sep_map_set_conj[symmetric] distinct_zipI1
+                   simp flip: map_nth_length[where xs=ids]
+                              map_nth_length[where xs="zip cptrs' caps'" for cptrs' caps']
+                   intro: map_sep_list_conj_cong)
   done
 
 lemma make_untyped_map_find:
@@ -1051,12 +1088,12 @@ lemma lookup_cptr_wp:
   apply (clarsimp simp: make_untyped_map_find zip_map_fst_snd opt_map_def)
   done
 
-declare is_full_untyped_cap_is_untyped_cap[simp]
-
 lemma retype_untypeds_wp_helper:
   defines
     "allocation_map spec untyped_map untyped_derivations \<equiv>
-       map (\<lambda>(parent, children). is (aligned_allocations spec ((Min o available_range \<circ> cap_of \<circ> untyped_map) parent) children))
+       map (\<lambda>(parent, children). (=) (aligned_allocations spec
+                                        ((Min o available_range \<circ> cap_of \<circ> untyped_map) parent)
+                                        children))
            untyped_derivations"
   shows
     "\<lbrakk>well_formed spec;
@@ -1074,17 +1111,20 @@ lemma retype_untypeds_wp_helper:
                 object_size_bits (the (cdl_objects spec child)) < 2 ^ word_bits \<and>
                 Min (available_range (cap_of (untyped_map (fst x))))
                 \<le> Min (available_range (cap_of (untyped_map (fst x)))) +
-                   2 ^ obj_bits_cdl (object_type (the (cdl_objects spec child))) (object_size_bits (the (cdl_objects spec child))) \<and>
-                obj_bits_cdl (object_type (the (cdl_objects spec child))) (object_size_bits (the (cdl_objects spec child))) < word_size)
+                   2 ^ obj_bits_cdl (object_type (the (cdl_objects spec child)))
+                                    (object_size_bits (the (cdl_objects spec child))) \<and>
+                obj_bits_cdl (object_type (the (cdl_objects spec child)))
+                             (object_size_bits (the (cdl_objects spec child))) < word_size)
         untyped_derivations;
       list_all (\<lambda>n. n < 2 ^ si_cnode_size) untyped_slots;
       list_all (\<lambda>n. n < 2 ^ si_cnode_size) (list_region free_cptrs);
       list_all (\<lambda>d. list_all
-              (\<lambda>child.
-                  previous child (snd d) \<noteq> None \<longrightarrow>
-                  Min ((available_range \<circ> cap_of \<circ> untyped_map \<circ> fst) d)
-                  < the (allocate ((Min o available_range \<circ> cap_of \<circ> untyped_map o fst)  d) spec (snd d) child))
-              (snd d)) untyped_derivations;
+                      (\<lambda>child.
+                          previous child (snd d) \<noteq> None \<longrightarrow>
+                          Min ((available_range \<circ> cap_of \<circ> untyped_map \<circ> fst) d)
+                          < the (allocate ((Min o available_range \<circ> cap_of \<circ> untyped_map o fst) d)
+                                           spec (snd d) child))
+                      (snd d)) untyped_derivations;
       list_all (\<lambda>cap. available_range cap \<noteq> {}) untyped_caps;
        list_all (\<lambda>d.
          \<forall>child\<in>set (snd d).
@@ -1092,12 +1132,14 @@ lemma retype_untypeds_wp_helper:
                 \<in> available_range (cap_of (untyped_map (fst d)))) untyped_derivations;
       list_all (\<lambda>d. let cover_ids = (Min o available_range \<circ> cap_of \<circ> untyped_map  o fst) d in
                     list_all (\<lambda>child. cover_ids
-                    \<le> the (aligned_allocations spec cover_ids (snd d) child) + 2 ^ spec_object_size spec child) (snd d))
+                                        \<le> the (aligned_allocations spec cover_ids (snd d) child) +
+                                          2 ^ spec_object_size spec child) (snd d))
                 untyped_derivations;
       list_all
         (\<lambda>x. \<forall>child\<in>set (snd x).
                 is_aligned (Min (available_range (cap_of (untyped_map (fst x)))))
-                 (obj_bits_cdl (object_type (the (cdl_objects spec child))) (object_size_bits (the (cdl_objects spec child)))))
+                           (obj_bits_cdl (object_type (the (cdl_objects spec child)))
+                                         (object_size_bits (the (cdl_objects spec child)))))
         untyped_derivations;
       valid_untypeds (map fst untyped_derivations) (map fst untyped_list)
                      (map snd untyped_list) untyped_caps;
@@ -1113,13 +1155,15 @@ lemma retype_untypeds_wp_helper:
     distinct_sets (map (set o snd) untyped_derivations)\<rbrace>
    create_objects spec untyped_list free_cptrs (untyped_derivations :: (machine_word \<times> (machine_word list)) list)
    \<lbrace>\<lambda>(si_caps', free_cptrs') s.
-     \<guillemotleft>\<And>* map (\<lambda>(slot, cap). on_depleted_untyped_cap (sep_map_c (si_cnode_id, unat slot)) cap) (zip untyped_slots untyped_caps) \<and>*
+     \<guillemotleft>\<And>* map (\<lambda>(slot, cap). on_depleted_untyped_cap (sep_map_c (si_cnode_id, unat slot)) cap)
+             (zip untyped_slots untyped_caps) \<and>*
       objects_empty spec t (set (collect_children untyped_derivations)) \<and>*
       si_caps_at t si_caps spec dev (set (collect_children untyped_derivations)) \<and>*
       si_objects \<and>* R\<guillemotright> s \<and>
      si_caps = si_caps' \<and>
      free_cptrs' = drop_region (length (collect_children untyped_derivations)) free_cptrs\<rbrace>"
   supply list_all_iff[simp] map_of_zip_is_Some'[symmetric, simp] split_beta'[simp]
+  supply is_full_untyped_cap_is_untyped_cap[simp]
   apply (rule hoare_name_pre_state)
   apply (unfold create_objects_def)
   apply (clarsimp simp: valid_untypeds_def)
@@ -1128,23 +1172,24 @@ lemma retype_untypeds_wp_helper:
    apply (clarsimp split: prod.splits)
    apply (frule (1) distinct_fst_snd_distinct)
    apply (rule sep_hoare_fold_mapM_x, rule bind_wp,
-          rule create_children_wp[where dev=dev and t="t" and
-                                        cover_ids ="(available_range o cap_of o untyped_map o fst) v" and
-                                        parent_cptr'="cptr_of (untyped_map (fst v))"
-                                  for v, simplified sep_wp_simp];
-          try_solves \<open>simp\<close>)
+          rule create_children_wp[where dev = dev
+                                    and t="t"
+                                    and cover_ids = "(available_range \<circ> cap_of \<circ> untyped_map \<circ> fst) v"
+                                    and parent_cptr'="cptr_of (untyped_map (fst v))" for v,
+                                  simplified sep_wp_simp];
+          (solves simp)?)
            apply (simp add: Let_unfold)
            apply (erule (1) bspec)
           apply simp
           apply meson
-         apply (clarsimp simp: allocation_map_def)
+         apply (clarsimp simp: allocation_map_def map_allocates)
         apply (simp, erule bspec)
         apply (rule cap_of_make_untyped_map[simplified]; clarsimp)
        apply (fastforce)
       apply (clarsimp)
-      apply (rule the_map_of_elim; clarsimp?)
+      apply (rule the_map_of_elim; (clarsimp simp: child_in_collection)?)
       apply (meson in_set_takeD)
-     apply clarsimp+
+     apply (clarsimp)+
    apply wpfix
    apply (rule hoare_weaken_pre)
     apply (erule lookup_cptr_wp; clarsimp)
@@ -1162,14 +1207,18 @@ lemma retype_untypeds_wp_helper:
   apply clarsimp
   apply (sep_fold_cancel)+
   apply (rule sep_map_sep_foldI)
-  apply (subgoal_tac "set (collect_children untyped_derivations) = (\<Union>x\<in>set untyped_derivations. set (snd x))")
-   apply (clarsimp simp: sep_list_conj_sep_map_set_conj distinct_zipI1 distinct_map_comp[where f=unat] unat_inj distinct_map_comp'  )
+  apply (subgoal_tac "set (collect_children untyped_derivations) =
+                      (\<Union>x\<in>set untyped_derivations. set (snd x))")
+   apply (clarsimp simp: sep_list_conj_sep_map_set_conj
+                         distinct_zipI1 distinct_map_comp[where f=unat] unat_inj distinct_map_comp')
    apply (clarsimp simp: si_null_caps_at_def si_caps_at_def objects_empty_def)
-   apply (clarsimp simp: sep_map_set_squash[OF untyped_derivations_inject, simplified]  sep_map_set_conj_Union[OF _ helper])
+   apply (clarsimp simp: sep_map_set_squash[OF untyped_derivations_inject, simplified]
+                         sep_map_set_conj_Union[OF _ distinct_sets_helper])
    apply (sep_cancel)+
-   apply (comp_folder comp: comp_folder[where g=fst])+
+   apply (subst sep_map_set_conj_fold_fst)+
    apply (simp only: sep.prod.reindex[symmetric, where h=fst, OF distinct_inj_on])
-   apply (subst sep_prod_make_untyped_map_zip[where ids="map fst untyped_derivations", simplified]; clarsimp)+
+   apply (subst sep_prod_make_untyped_map_zip[where ids="map fst untyped_derivations", simplified];
+          clarsimp)+
    apply (erule (1) sep_conj_impl[OF _ sep_map_set_conj_impl[simplified]]; clarsimp?)
     apply (erule back_subst[OF _ untyped_cap_helper[symmetric]]; fastforce elim!: in_set_zipE)
    apply (sep_cancel)+
@@ -1187,11 +1236,9 @@ lemma retype_untypeds_wp_helper:
   done
 
 lemma real_object_at_inter_cdl_objects [simp]:
-  "{obj_id. real_object_at obj_id spec} \<inter> dom (cdl_objects spec) = {obj_id. real_object_at obj_id spec}"
+  "{obj_id. real_object_at obj_id spec} \<inter> dom (cdl_objects spec) =
+   {obj_id. real_object_at obj_id spec}"
   by (auto simp: real_object_at_def)
-
-lemma map_of_nat_unat: "map of_nat (map unat xs) = xs"
-  by (clarsimp)
 
 lemma create_objects_sep:
   "\<lbrace> \<guillemotleft>\<And>* map  (\<lambda>(slot, cap).  (sep_map_c (si_cnode_id, slot)) cap) (zip untyped_slots untyped_caps) \<and>*
@@ -1231,106 +1278,97 @@ lemma create_objects_sep:
                       apply (fastforce)
                      apply (assumption | rule refl)+
                 apply (clarsimp simp: valid_derivations_def Let_unfold list_all_iff)
-                apply (drule_tac x="(a,b)" in bspec, assumption, clarsimp, drule_tac x=child in  bspec, assumption )
+                apply (rename_tac a b child)
+                apply (drule_tac x="(a,b)" in bspec, assumption, clarsimp)
+                apply (drule_tac x=child in bspec, assumption)
                 apply (clarsimp simp: spec_object_size_def)
                apply (fastforce simp: unat_less_2_si_cnode_size list_all_iff)
               apply clarsimp
              apply (clarsimp simp: valid_derivations_def valid_untypeds_def Let_unfold list_all_iff)+
-         apply (drule_tac x="(a,b)" in bspec, assumption, clarsimp, drule_tac x=child in  bspec, assumption )
+         apply (rename_tac a b child)
+         apply (drule_tac x="(a,b)" in bspec, assumption, clarsimp)
+         apply (drule_tac x=child in bspec, assumption)
          apply (clarsimp simp: spec_object_size_def)
         apply clarsimp
        apply (clarsimp simp: valid_derivations_def Let_unfold list_all_iff)
        apply (rule refl)
       apply (clarsimp simp: valid_derivations_def Let_unfold list_all_iff)+
-   apply (fastforce simp: zip_map_map comp_def apfst_def map_prod_def)+
+   apply (fastforce simp: zip_map_eq_map comp_def apfst_def map_prod_def)+
   done
 
-lemma map_of_zip_not_none: "x \<in> set xs \<Longrightarrow> length xs \<le> length ys \<Longrightarrow> map_of (zip xs ys) x \<noteq> None"
+lemma map_of_zip_not_None: (* FIXME: move to Lib *)
+  "\<lbrakk> x \<in> set xs; length xs \<le> length ys \<rbrakk> \<Longrightarrow> map_of (zip xs ys) x \<noteq> None"
   apply (induct xs; clarsimp)
-  apply (case_tac ys; clarsimp)
-  by (simp add: map_of_zip_is_Some')
+  apply (case_tac ys; clarsimp simp: map_of_zip_is_Some')
+  done
 
-
-lemma sep_map_set_conj_set_append: "distinct (xs@ys) \<Longrightarrow> sep_map_set_conj P (set (xs @ ys)) = (sep_map_set_conj P (set xs) \<and>* sep_map_set_conj P (set ys))"
- apply (induct xs; clarsimp)
- apply (case_tac ys; clarsimp)
- apply (rule ext; rule iffI; sep_solve)
-done
-
-lemma sep_map_set_conj_set_take_drop: "sep_map_set_conj P (set xs) s \<Longrightarrow> distinct xs \<Longrightarrow> (sep_map_set_conj P (set (take n xs)) \<and>*  sep_map_set_conj P (set (drop n xs))) s"
- by (clarsimp simp: append_take_drop_id[where n=n, symmetric] sep_map_set_conj_set_append[symmetric]  )
-
-
-
-
-
-
-lemma map2_map_left: "map2 (\<lambda>x. f (g x)) xs ys = map2 f (map g xs) ys"
+lemma map2_map_left: (* FIXME: move to Lib *)
+  "map2 (\<lambda>x. f (g x)) xs ys = map2 f (map g xs) ys"
   apply (induct xs arbitrary:ys ; clarsimp)
   apply (case_tac ys; clarsimp)
   done
 
-lemma filter_notin: "\<not> x \<in> set xs \<Longrightarrow> filter (\<lambda>y. y \<noteq> x) xs = xs"
+lemma filter_notin: (* FIXME: move to Lib *)
+  "\<not> x \<in> set xs \<Longrightarrow> filter (\<lambda>y. y \<noteq> x) xs = xs"
   by (induct xs; clarsimp)
 
-lemma sep_map_map_of: "\<lbrakk>length xs \<le> length ys; distinct xs; distinct ys\<rbrakk> \<Longrightarrow>
-      (SETSEPCONJ x:set xs. f (the (map_of (zip xs ys) x))) = (SETSEPCONJ x:set (take (length xs) ys). f x)"
+lemma sep_map_map_of:
+  "\<lbrakk>length xs \<le> length ys; distinct xs; distinct ys\<rbrakk> \<Longrightarrow>
+   (SETSEPCONJ x:set xs. f (the (map_of (zip xs ys) x))) =
+   (SETSEPCONJ x:set (take (length xs) ys). f x)"
   apply (induct xs arbitrary:ys; clarsimp)
-  apply (case_tac ys; clarsimp)
-  apply (subst sep.prod.insert_remove)
-   apply (clarsimp)
-  apply (clarsimp)
+  apply (rename_tac ys, case_tac ys; clarsimp)
+  apply (clarsimp simp: sep.prod.insert_remove)
   apply (subst set_minus_filter_out)
   apply (subst filter_notin)
    apply (clarsimp)
    apply (meson in_set_takeD)
-  apply (subst sep_map_set_conj_subst[OF arg_cong])
-   apply (rule_tac s="the (map_of (zip xs list) x)" in sym)
-   apply (clarsimp)
-  apply (drule_tac x=list in meta_spec)
-  apply (clarsimp)
+  apply (smt (verit, best) sep.prod.cong)
   done
 
 lemma si_null_cap_at_unfold:
   "\<lbrakk>cap_map obj_id \<noteq> None; the (cap_map obj_id) < 2 ^ si_cnode_size;
     cdl_objects spec obj_id \<noteq> None; t obj_id \<noteq> None\<rbrakk> \<Longrightarrow>
-  si_null_cap_at t cap_map spec obj_id = (si_cnode_id, unat (the (cap_map obj_id))) \<mapsto>c NullCap"
+   si_null_cap_at t cap_map spec obj_id = (si_cnode_id, unat (the (cap_map obj_id))) \<mapsto>c NullCap"
   by (rule ext, clarsimp simp: si_null_cap_at_def)
 
-lemma [simp]: "collect_children ((a, b) # xs) = b @ collect_children xs"
+lemma collect_children_Cons[simp]:
+  "collect_children ((a, b) # xs) = b @ collect_children xs"
   by (clarsimp simp: collect_children_def)
 
-lemma distinct_collection': "distinct_sets (map (set o snd) xs) \<Longrightarrow> list_all distinct (map snd xs) \<Longrightarrow> distinct (collect_children xs)"
+lemma distinct_collection':
+  "\<lbrakk> distinct_sets (map (set \<circ> snd) xs); list_all distinct (map snd xs) \<rbrakk> \<Longrightarrow>
+  distinct (collect_children xs)"
   apply (induct xs; clarsimp)
    apply (clarsimp simp: collect_children_def)
   apply (erule disjoint_subset2[rotated])
   apply (simp add: collect_children_def set_list_bind)
   done
 
-lemma distinct_collection[simp]: "valid_derivations spec untyped_derivations untyped_caps \<Longrightarrow> distinct (collect_children untyped_derivations)"
+lemma distinct_collection:
+  "valid_derivations spec untyped_derivations untyped_caps \<Longrightarrow>
+   distinct (collect_children untyped_derivations)"
   apply (rule distinct_collection')
    apply (clarsimp simp: valid_derivations_def)
   apply (clarsimp simp: valid_derivations_def Let_unfold)
   apply (simp add: list_all_iff)
   done
 
-lemma is_in_sep_list_conjD': "sep_list_conj (map (\<lambda>x. is (g x)) xs) s \<Longrightarrow> \<exists>x. x \<in> set xs \<and> v \<in> dom (g x) \<Longrightarrow> s v \<noteq> None "
-  apply (clarsimp)
-  apply (subst (asm) sep_list_conj_map_remove1, assumption)
-  apply (drule  is_in_rangeD)
-   apply (fastforce simp: dom_def)+
-  done
+lemma is_in_sep_list_conjD':
+  "\<lbrakk> sep_list_conj (map (\<lambda>x. (=) (g x)) xs) s; \<exists>x. x \<in> set xs \<and> v \<in> dom (g x) \<rbrakk> \<Longrightarrow> s v \<noteq> None "
+  by (fastforce dest: is_in_rangeD simp: sep_list_conj_map_remove1)
 
-lemma in_collection_in_derivations: "x \<in> set (collect_children untyped_derivations) \<Longrightarrow>
-    \<exists>parent family. x\<in> set family \<and> (parent, family) \<in> set untyped_derivations"
+lemma in_collection_in_derivations:
+  "x \<in> set (collect_children untyped_derivations) \<Longrightarrow>
+   \<exists>parent family. x\<in> set family \<and> (parent, family) \<in> set untyped_derivations"
   apply (induct untyped_derivations; clarsimp simp: collect_children_def List.bind_def)
   apply blast
   done
 
 lemma create_objects_sep':
-  "\<lbrace> \<guillemotleft>\<And>* map  (\<lambda>(slot, cap).  (sep_map_c (si_cnode_id, unat slot)) cap) (zip untyped_slots untyped_caps) \<and>*
-      (\<And>* cptr\<in>set_region free_cptrs.
-            (si_cnode_id, unat cptr) \<mapsto>c NullCap) \<and>*
+  "\<lbrace> \<guillemotleft>\<And>* map (\<lambda>(slot, cap). (sep_map_c (si_cnode_id, unat slot)) cap)
+             (zip untyped_slots untyped_caps) \<and>*
+      (\<And>* cptr\<in>set_region free_cptrs. (si_cnode_id, unat cptr) \<mapsto>c NullCap) \<and>*
       (\<And>* obj_id\<in>(set (collect_children untyped_derivations)). the (t obj_id) \<mapsto>o Untyped) \<and>*
       si_objects \<and>* R\<guillemotright> and
      K (well_formed spec \<and>
@@ -1346,73 +1384,69 @@ lemma create_objects_sep':
         map fst untyped_list = untyped_slots \<and>
         (\<forall>obj\<in>ran (cdl_objects spec). object_domain obj = minBound) \<and>
         (\<And>* map (\<lambda>(parent, children).
-                   (=) (aligned_allocations spec ((Min \<circ> available_range \<circ> cap_of \<circ> untyped_map) parent)
+                   (=) (aligned_allocations spec
+                                            ((Min \<circ> available_range \<circ> cap_of \<circ> untyped_map) parent)
                                             children))
                 untyped_derivations) t \<and>
         length (collect_children untyped_derivations) \<le> length_region free_cptrs \<and>
         valid_slot_region free_cptrs)\<rbrace>
-   create_objects spec untyped_list free_cptrs (untyped_derivations :: (machine_word \<times> (machine_word list)) list)
+   create_objects spec untyped_list free_cptrs
+                  (untyped_derivations :: (machine_word \<times> machine_word list) list)
    \<lbrace>\<lambda>_ s.
-     \<guillemotleft>\<And>* map (\<lambda>(slot, cap). on_depleted_untyped_cap (sep_map_c (si_cnode_id, unat slot)) cap) (zip untyped_slots untyped_caps) \<and>*
+     \<guillemotleft>\<And>* map (\<lambda>(slot, cap). on_depleted_untyped_cap (sep_map_c (si_cnode_id, unat slot)) cap)
+             (zip untyped_slots untyped_caps) \<and>*
       objects_empty spec t (set (collect_children untyped_derivations)) \<and>*
-      si_caps_at t (map_of (zip_region (collect_children untyped_derivations) free_cptrs)) spec dev (set (collect_children untyped_derivations)) \<and>*
+      si_caps_at t (map_of (zip_region (collect_children untyped_derivations) free_cptrs)) spec dev
+                   (set (collect_children untyped_derivations)) \<and>*
       (\<And>* cptr\<in>set_region (drop_region (length (collect_children untyped_derivations)) free_cptrs).
             (si_cnode_id, unat cptr) \<mapsto>c NullCap) \<and>*
       si_objects  \<and>* R\<guillemotright> s\<rbrace>"
-  apply (rule hoare_chain[OF create_objects_sep[where untyped_caps=untyped_caps and
-                                                      untyped_slots="(map (unat o fst) untyped_list)" and
-                                                      untyped_map=untyped_map]];
-         clarsimp simp: pred_conj_def)
-   defer
-   apply (sep_solve)
+   apply (rule create_objects_sep[where untyped_caps=untyped_caps and
+                                        untyped_slots="(map (unat \<circ> fst) untyped_list)" and
+                                        untyped_map=untyped_map,
+                                  THEN hoare_chain];
+          clarsimp simp: pred_conj_def)
   apply (intro conjI)
-       defer
+       defer (* schematic *)
        apply (fastforce)
       apply (clarsimp simp: list_all_iff)
-  using unat_less_2_si_cnode_size' apply auto[1]
+      apply (auto simp: unat_less_2_si_cnode_size')[1]
      apply (fastforce)
     apply (fastforce simp: valid_untypeds_def)
    apply (clarsimp simp: valid_untypeds_def, sep_cancel+)
   apply (erule sep_conj_impl)
    apply (subst (asm) map2_map_left[where g=unat])
    apply (clarsimp)
-  apply (sep_drule sep_map_set_conj_set_take_drop[where n="length (collect_children untyped_derivations)"])
+  apply (sep_drule sep_map_set_conj_set_take_drop[where
+                     n="length (collect_children untyped_derivations)"])
    apply (clarsimp)
   apply (sep_flatten)
   apply (erule sep_conj_impl)
    defer
    apply (sep_cancel)+
    apply (subst  map2_map_left[where g=unat], clarsimp)
-  apply (clarsimp simp: comp_def)
-  apply (clarsimp simp: list_all_iff)
-  apply (clarsimp simp: si_null_caps_at_def)
+  apply (clarsimp simp: comp_def list_all_iff si_null_caps_at_def)
   apply (subst sep_map_set_conj_subst[OF si_null_cap_at_unfold])
-      apply (simp add: map_of_zip_not_none)
+      apply (simp add: map_of_zip_not_None)
      prefer 4
-     apply (subst sep_map_map_of; clarsimp?)
+     apply (subst sep_map_map_of; (clarsimp simp: distinct_collection)?)
     apply (erule valid_slot_region_less)
     apply (rule set_rev_mp)
      apply (rule the_map_of_zip_inR; clarsimp)
     apply (simp add: set_take_subset)
    defer
-   apply (rule_tac is_in_sep_list_conjD'[where xs=untyped_derivations and
-                                               g="\<lambda>(parent, children). (aligned_allocations spec
-                                                  ((Min o available_range \<circ> cap_of \<circ> untyped_map)
-                                                  parent) children)" and
-                                               s=t])
-    apply (clarsimp)
-    apply (simp add: prod_lift_lambda)
-   apply (clarsimp)
-   apply (frule in_collection_in_derivations, clarsimp)
-   apply (rule exI)+
-   apply (intro conjI)
-    apply (fastforce)
-   apply (clarsimp)
-   apply (clarsimp simp: aligned_allocations_def)
-   apply (rule exI)
-   apply (rule mapp_app)
-   apply (simp add: in_list_allocate)
-  apply (clarsimp simp: dom_def)
+   apply (rule_tac is_in_sep_list_conjD'[where
+                     xs = untyped_derivations and
+                     g = "\<lambda>(p, cs). aligned_allocations
+                                      spec
+                                      ((Min o available_range \<circ> cap_of \<circ> untyped_map) p)
+                                      cs" and
+                     s = t])
+    apply (clarsimp simp: split_def)
+   apply (fastforce intro: mapp_app
+                    dest: in_collection_in_derivations
+                    simp: in_list_allocate aligned_allocations_def)
+  apply (clarsimp)
   apply (drule (1) set_rev_mp)
   apply (clarsimp)
   done
